theories/parabstr/ws_hub_1.v
@@ -21,7 +21,7 @@ From zebre.std Require Import
 From zebre.saturn Require Import
   mpmc_queue_1.
 From zebre.parabstr Require Export
-  base.
+  ws_hub.
 From zebre.parabstr Require Import
   ws_deques
   waiters.
@@ -54,7 +54,7 @@ Section ws_deques.
   Context `{zebre_G : !ZebreG Σ}.
   Context (ws_deques : ws_deques Σ).
 
-  Definition ws_hub_create : val :=
+  Definition ws_hub_1_create : val :=
     λ: "sz",
       { ws_deques.(ws_deques_create) "sz";
         mpmc_queue_create ();
@@ -62,239 +62,221 @@ Section ws_deques.
         waiters_create ()
       }.
 
-  #[local] Definition ws_hub_notify : val :=
+  #[local] Definition ws_hub_1_notify : val :=
     λ: "t",
       waiters_notify "t".{waiters}.
 
-  Definition ws_hub_push : val :=
+  Definition ws_hub_1_push : val :=
     λ: "t" "i" "v",
       ws_deques.(ws_deques_push) "t".{deques} "i" "v" ;;
-      ws_hub_notify "t".
+      ws_hub_1_notify "t".
 
   #[using="ws_deques"]
-  Definition ws_hub_push_foreign : val :=
+  Definition ws_hub_1_push_foreign : val :=
     λ: "t" "v",
       mpmc_queue_push "t".{foreign} "v" ;;
-      ws_hub_notify "t".
+      ws_hub_1_notify "t".
 
-  Definition ws_hub_pop : val :=
+  Definition ws_hub_1_pop : val :=
     λ: "t" "i",
       ws_deques.(ws_deques_pop) "t".{deques} "i".
 
-  #[local] Definition ws_hub_pop_foreign : val :=
+  #[local] Definition ws_hub_1_pop_foreign : val :=
     λ: "t",
       mpmc_queue_pop "t".{foreign}.
 
-  #[local] Definition ws_hub_try_steal_once : val :=
+  #[local] Definition ws_hub_1_try_steal_once : val :=
     λ: "t" "i",
       let: "round" := array_unsafe_get "t".{rounds} "i" in
       random_round_reset "round" ;;
       ws_deques_steal_as ws_deques "t".{deques} "i" "round".
 
-  #[local] Definition ws_hub_try_steal_aux yield : val :=
-    rec: "ws_hub_try_steal_aux" "t" "i" "max_round" :=
+  #[local] Definition ws_hub_1_try_steal_aux yield : val :=
+    rec: "ws_hub_1_try_steal_aux" "t" "i" "max_round" :=
       if: "max_round" ≤ #0 then (
         §None
       ) else (
-        match: ws_hub_pop_foreign "t" with
+        match: ws_hub_1_pop_foreign "t" with
         | Some <> as "res" =>
             "res"
         | None =>
-            match: ws_hub_try_steal_once "t" "i" with
+            match: ws_hub_1_try_steal_once "t" "i" with
             | Some <> as "res" =>
                 "res"
             | None =>
                 (if yield then Yield else ()) ;;
-                "ws_hub_try_steal_aux" "t" "i" ("max_round" - #1)
+                "ws_hub_1_try_steal_aux" "t" "i" ("max_round" - #1)
             end
         end
       ).
-  Definition ws_hub_try_steal : val :=
+  Definition ws_hub_1_try_steal : val :=
     λ: "t" "i" "max_round",
-      match: ws_hub_try_steal_aux false "t" "i" "max_round".<0> with
+      match: ws_hub_1_try_steal_aux false "t" "i" "max_round".<0> with
       | Some <> as "res" =>
           "res"
       | None =>
-          ws_hub_try_steal_aux true "t" "i" "max_round".<1>
+          ws_hub_1_try_steal_aux true "t" "i" "max_round".<1>
       end.
 
-  Definition ws_hub_pop_try_steal : val :=
-    λ: "t" "i" "max_round",
-      match: ws_hub_pop "t" "i" with
-      | Some <> as "res" =>
-          "res"
-      | None =>
-          ws_hub_try_steal "t" "i" "max_round"
-      end.
-
-  Definition ws_hub_steal : val :=
-    rec: "ws_hub_steal" "t" "i" "max_round" :=
-      match: ws_hub_try_steal "t" "i" "max_round" with
+  Definition ws_hub_1_steal : val :=
+    rec: "ws_hub_1_steal" "t" "i" "max_round" :=
+      match: ws_hub_1_try_steal "t" "i" "max_round" with
       | Some "v" =>
           "v"
       | None =>
           let: "waiters" := "t".{waiters} in
           let: "waiter" := waiters_prepare_wait "waiters" in
-          match: ws_hub_try_steal_once "t" "i" with
+          match: ws_hub_1_try_steal_once "t" "i" with
           | Some "v" =>
               waiters_cancel_wait "waiters" "waiter" ;;
               "v"
           | None =>
               waiters_commit_wait "waiters" "waiter" ;;
-              "ws_hub_steal" "t" "i" "max_round"
+              "ws_hub_1_steal" "t" "i" "max_round"
           end
-      end.
-
-  Definition ws_hub_pop_steal : val :=
-    λ: "t" "i" "max_round",
-      match: ws_hub_pop "t" "i" with
-      | Some "v" =>
-          "v"
-      | None =>
-          ws_hub_steal "t" "i" "max_round"
       end.
 End ws_deques.
 
-Class WsHubG Σ `{zebre_G : !ZebreG Σ} := {
-  #[local] ws_hub_G_queue_G :: MpmcQueueG Σ ;
-  #[local] ws_hub_G_waiters_G :: WaitersG Σ ;
-  #[local] ws_hub_G_model_G :: TwinsG Σ (leibnizO (gmultiset val)) ;
+Class WsHub1G Σ `{zebre_G : !ZebreG Σ} := {
+  #[local] ws_hub_1_G_queue_G :: MpmcQueueG Σ ;
+  #[local] ws_hub_1_G_waiters_G :: WaitersG Σ ;
+  #[local] ws_hub_1_G_model_G :: TwinsG Σ (leibnizO (gmultiset val)) ;
 }.
 
-Definition ws_hub_Σ := #[
+Definition ws_hub_1_Σ := #[
   mpmc_queue_Σ ;
   waiters_Σ ;
   twins_Σ (leibnizO (gmultiset val))
 ].
-#[global] Instance subG_ws_hub_Σ Σ `{zebre_G : !ZebreG Σ} :
-  subG ws_hub_Σ Σ →
-  WsHubG Σ.
+#[global] Instance subG_ws_hub_1_Σ Σ `{zebre_G : !ZebreG Σ} :
+  subG ws_hub_1_Σ Σ →
+  WsHub1G Σ.
 Proof.
   solve_inG.
 Qed.
 
-Section ws_hub_G.
-  Context `{ws_hub_G : WsHubG Σ}.
+Section ws_hub_1_G.
+  Context `{ws_hub_1_G : WsHub1G Σ}.
   Context (ws_deques : ws_deques Σ).
 
-  Record ws_hub_meta := {
-    ws_hub_meta_size : nat ;
-    ws_hub_meta_deques : val ;
-    ws_hub_meta_foreign : val ;
-    ws_hub_meta_rounds : val ;
-    ws_hub_meta_waiters : val ;
-    ws_hub_meta_model : gname ;
+  Record ws_hub_1_meta := {
+    ws_hub_1_meta_size : nat ;
+    ws_hub_1_meta_deques : val ;
+    ws_hub_1_meta_foreign : val ;
+    ws_hub_1_meta_rounds : val ;
+    ws_hub_1_meta_waiters : val ;
+    ws_hub_1_meta_model : gname ;
   }.
-  Implicit Types γ : ws_hub_meta.
+  Implicit Types γ : ws_hub_1_meta.
 
-  #[local] Instance ws_hub_meta_eq_dec :
-    EqDecision ws_hub_meta.
+  #[local] Instance ws_hub_1_meta_eq_dec :
+    EqDecision ws_hub_1_meta.
   Proof.
     solve_decision.
   Qed.
-  #[local] Instance ws_hub_meta_countable :
-    Countable ws_hub_meta.
+  #[local] Instance ws_hub_1_meta_countable :
+    Countable ws_hub_1_meta.
   Proof.
     pose encode γ := (
-      γ.(ws_hub_meta_size),
-      γ.(ws_hub_meta_deques),
-      γ.(ws_hub_meta_foreign),
-      γ.(ws_hub_meta_rounds),
-      γ.(ws_hub_meta_waiters),
-      γ.(ws_hub_meta_model)
+      γ.(ws_hub_1_meta_size),
+      γ.(ws_hub_1_meta_deques),
+      γ.(ws_hub_1_meta_foreign),
+      γ.(ws_hub_1_meta_rounds),
+      γ.(ws_hub_1_meta_waiters),
+      γ.(ws_hub_1_meta_model)
     ).
     pose decode := λ '(γ_size, γ_deques, γ_foreign, γ_rounds, γ_waiters, γ_model), {|
-      ws_hub_meta_size := γ_size ;
-      ws_hub_meta_deques := γ_deques ;
-      ws_hub_meta_foreign := γ_foreign ;
-      ws_hub_meta_rounds := γ_rounds ;
-      ws_hub_meta_waiters := γ_waiters ;
-      ws_hub_meta_model := γ_model ;
+      ws_hub_1_meta_size := γ_size ;
+      ws_hub_1_meta_deques := γ_deques ;
+      ws_hub_1_meta_foreign := γ_foreign ;
+      ws_hub_1_meta_rounds := γ_rounds ;
+      ws_hub_1_meta_waiters := γ_waiters ;
+      ws_hub_1_meta_model := γ_model ;
     |}.
     refine (inj_countable' encode decode _). intros []. done.
   Qed.
 
-  #[local] Definition ws_hub_model₁' γ_model vs :=
+  #[local] Definition ws_hub_1_model₁' γ_model vs :=
     twins_twin1 γ_model (DfracOwn 1) vs.
-  #[local] Definition ws_hub_model₁ γ vs :=
-    ws_hub_model₁' γ.(ws_hub_meta_model) vs.
-  #[local] Definition ws_hub_model₂' γ_model vs :=
+  #[local] Definition ws_hub_1_model₁ γ vs :=
+    ws_hub_1_model₁' γ.(ws_hub_1_meta_model) vs.
+  #[local] Definition ws_hub_1_model₂' γ_model vs :=
     twins_twin2 γ_model vs.
-  #[local] Definition ws_hub_model₂ γ vs :=
-    ws_hub_model₂' γ.(ws_hub_meta_model) vs.
+  #[local] Definition ws_hub_1_model₂ γ vs :=
+    ws_hub_1_model₂' γ.(ws_hub_1_meta_model) vs.
 
-  #[local] Definition ws_hub_inv_inner γ : iProp Σ :=
+  #[local] Definition ws_hub_1_inv_inner γ : iProp Σ :=
     ∃ vs vss vs_foreign,
     ⌜vs = foldr (λ vs_deques vs, list_to_set_disj vs_deques ⊎ vs) (list_to_set_disj vs_foreign) vss⌝ ∗
-    ws_deques.(ws_deques_model) γ.(ws_hub_meta_deques) vss ∗
-    mpmc_queue_model γ.(ws_hub_meta_foreign) vs_foreign ∗
-    ws_hub_model₂ γ vs.
-  Definition ws_hub_inv t ι : iProp Σ :=
+    ws_deques.(ws_deques_model) γ.(ws_hub_1_meta_deques) vss ∗
+    mpmc_queue_model γ.(ws_hub_1_meta_foreign) vs_foreign ∗
+    ws_hub_1_model₂ γ vs.
+  Definition ws_hub_1_inv t ι : iProp Σ :=
     ∃ l γ,
     ⌜t = #l⌝ ∗
     meta l nroot γ ∗
-    l.[deques] ↦□ γ.(ws_hub_meta_deques) ∗
-    l.[foreign] ↦□ γ.(ws_hub_meta_foreign) ∗
-    l.[waiters] ↦□ γ.(ws_hub_meta_waiters) ∗
-    ws_deques.(ws_deques_inv) γ.(ws_hub_meta_deques) (ι.@"deques") γ.(ws_hub_meta_size) ∗
-    mpmc_queue_inv γ.(ws_hub_meta_foreign) (ι.@"foreign") ∗
-    waiters_inv γ.(ws_hub_meta_waiters) ∗
-    inv (ι.@"inv") (ws_hub_inv_inner γ).
+    l.[deques] ↦□ γ.(ws_hub_1_meta_deques) ∗
+    l.[foreign] ↦□ γ.(ws_hub_1_meta_foreign) ∗
+    l.[waiters] ↦□ γ.(ws_hub_1_meta_waiters) ∗
+    ws_deques.(ws_deques_inv) γ.(ws_hub_1_meta_deques) (ι.@"deques") γ.(ws_hub_1_meta_size) ∗
+    mpmc_queue_inv γ.(ws_hub_1_meta_foreign) (ι.@"foreign") ∗
+    waiters_inv γ.(ws_hub_1_meta_waiters) ∗
+    inv (ι.@"inv") (ws_hub_1_inv_inner γ).
 
   #[using="ws_deques"]
-  Definition ws_hub_model t vs : iProp Σ :=
+  Definition ws_hub_1_model t vs : iProp Σ :=
     ∃ l γ,
     ⌜t = #l⌝ ∗
     meta l nroot γ ∗
-    ws_hub_model₁ γ vs.
+    ws_hub_1_model₁ γ vs.
 
-  Definition ws_hub_owner t i : iProp Σ :=
+  Definition ws_hub_1_owner t i : iProp Σ :=
     ∃ l γ round n,
     ⌜t = #l⌝ ∗
     meta l nroot γ ∗
-    l.[rounds] ↦□ γ.(ws_hub_meta_rounds) ∗
-    ws_deques.(ws_deques_owner) γ.(ws_hub_meta_deques) i ∗
-    array_slice γ.(ws_hub_meta_rounds) γ.(ws_hub_meta_size) i DfracDiscarded [round] ∗
-    random_round_model' round (γ.(ws_hub_meta_size) - 1) n.
+    l.[rounds] ↦□ γ.(ws_hub_1_meta_rounds) ∗
+    ws_deques.(ws_deques_owner) γ.(ws_hub_1_meta_deques) i ∗
+    array_slice γ.(ws_hub_1_meta_rounds) γ.(ws_hub_1_meta_size) i DfracDiscarded [round] ∗
+    random_round_model' round (γ.(ws_hub_1_meta_size) - 1) n.
 
-  #[global] Instance ws_hub_model_timeless t vs :
-    Timeless (ws_hub_model t vs).
+  #[global] Instance ws_hub_1_model_timeless t vs :
+    Timeless (ws_hub_1_model t vs).
   Proof.
     apply _.
   Qed.
-  #[global] Instance ws_hub_inv_persistent t ι :
-    Persistent (ws_hub_inv t ι).
+  #[global] Instance ws_hub_1_inv_persistent t ι :
+    Persistent (ws_hub_1_inv t ι).
   Proof.
     apply _.
   Qed.
 
-  #[local] Lemma ws_hub_model_alloc :
+  #[local] Lemma ws_hub_1_model_alloc :
     ⊢ |==>
       ∃ γ_model,
-      ws_hub_model₁' γ_model ∅ ∗
-      ws_hub_model₂' γ_model ∅.
+      ws_hub_1_model₁' γ_model ∅ ∗
+      ws_hub_1_model₂' γ_model ∅.
   Proof.
     apply twins_alloc'.
   Qed.
-  #[local] Lemma ws_hub_model_agree γ vs1 vs2 :
-    ws_hub_model₁ γ vs1 -∗
-    ws_hub_model₂ γ vs2 -∗
+  #[local] Lemma ws_hub_1_model_agree γ vs1 vs2 :
+    ws_hub_1_model₁ γ vs1 -∗
+    ws_hub_1_model₂ γ vs2 -∗
     ⌜vs1 = vs2⌝.
   Proof.
     apply: twins_agree_L.
   Qed.
-  #[local] Lemma ws_hub_model_update {γ vs1 vs2} vs :
-    ws_hub_model₁ γ vs1 -∗
-    ws_hub_model₂ γ vs2 ==∗
-      ws_hub_model₁ γ vs ∗
-      ws_hub_model₂ γ vs.
+  #[local] Lemma ws_hub_1_model_update {γ vs1 vs2} vs :
+    ws_hub_1_model₁ γ vs1 -∗
+    ws_hub_1_model₂ γ vs2 ==∗
+      ws_hub_1_model₁ γ vs ∗
+      ws_hub_1_model₂ γ vs.
   Proof.
     apply twins_update'.
   Qed.
 
-  Lemma ws_hub_owner_exclusive t i :
-    ws_hub_owner t i -∗
-    ws_hub_owner t i -∗
+  Lemma ws_hub_1_owner_exclusive t i :
+    ws_hub_1_owner t i -∗
+    ws_hub_1_owner t i -∗
     False.
   Proof.
     iIntros "(%l & %γ & %rounds & %n & -> & #Hmeta & _ & Howner1 & _) (%_l & %_γ & %_rounds & %_n & %Heq & #_Hmeta & _ & Howner2 & _)". injection Heq as <-.
@@ -302,16 +284,16 @@ Section ws_hub_G.
     iApply (ws_deques_owner_exclusive with "Howner1 Howner2").
   Qed.
 
-  Lemma ws_hub_create_spec ι sz :
+  Lemma ws_hub_1_create_spec ι sz :
     (0 ≤ sz)%Z →
     {{{ True }}}
-      ws_hub_create ws_deques #sz
+      ws_hub_1_create ws_deques #sz
     {{{ t,
       RET t;
-      ws_hub_inv t ι ∗
-      ws_hub_model t ∅ ∗
+      ws_hub_1_inv t ι ∗
+      ws_hub_1_model t ∅ ∗
       [∗ list] i ∈ seq 0 (Z.to_nat sz),
-        ws_hub_owner t i
+        ws_hub_1_owner t i
     }}}.
   Proof.
     set sz' := Z.to_nat sz.
@@ -337,15 +319,15 @@ Section ws_hub_G.
     iMod (pointsto_persist with "Hl_rounds") as "#Hl_rounds".
     iMod (pointsto_persist with "Hl_waiters") as "#Hl_waiters".
 
-    iMod ws_hub_model_alloc as "(%γ_model & Hmodel₁ & Hmodel₂)".
+    iMod ws_hub_1_model_alloc as "(%γ_model & Hmodel₁ & Hmodel₂)".
 
     pose γ := {|
-      ws_hub_meta_size := sz' ;
-      ws_hub_meta_deques := deques ;
-      ws_hub_meta_foreign := foreign ;
-      ws_hub_meta_rounds := v_rounds ;
-      ws_hub_meta_waiters := waiters ;
-      ws_hub_meta_model := γ_model ;
+      ws_hub_1_meta_size := sz' ;
+      ws_hub_1_meta_deques := deques ;
+      ws_hub_1_meta_foreign := foreign ;
+      ws_hub_1_meta_rounds := v_rounds ;
+      ws_hub_1_meta_waiters := waiters ;
+      ws_hub_1_meta_model := γ_model ;
     |}.
 
     iMod (meta_set _ _ γ with "Hmeta") as "#Hmeta"; first done.
@@ -365,11 +347,11 @@ Section ws_hub_G.
       rewrite Hrounds. iSteps.
   Qed.
 
-  #[local] Lemma ws_hub_notify_spec t ι :
+  #[local] Lemma ws_hub_1_notify_spec t ι :
     {{{
-      ws_hub_inv t ι
+      ws_hub_1_inv t ι
     }}}
-      ws_hub_notify t
+      ws_hub_1_notify t
     {{{
       RET (); True
     }}}.
@@ -380,19 +362,19 @@ Section ws_hub_G.
     wp_apply (waiters_notify_spec with "Hwaiters_inv HΦ").
   Qed.
 
-  Lemma ws_hub_push_spec t ι i v :
+  Lemma ws_hub_1_push_spec t ι i v :
     (0 ≤ i)%Z →
     <<<
-      ws_hub_inv t ι ∗
-      ws_hub_owner t (Z.to_nat i)
+      ws_hub_1_inv t ι ∗
+      ws_hub_1_owner t (Z.to_nat i)
     | ∀∀ vs,
-      ws_hub_model t vs
+      ws_hub_1_model t vs
     >>>
-      ws_hub_push ws_deques t #i v @ ↑ι
+      ws_hub_1_push ws_deques t #i v @ ↑ι
     <<<
-      ws_hub_model t ({[+v+]} ⊎ vs)
+      ws_hub_1_model t ({[+v+]} ⊎ vs)
     | RET ();
-      ws_hub_owner t (Z.to_nat i)
+      ws_hub_1_owner t (Z.to_nat i)
     >>>.
   Proof.
     iIntros "%Hi !> %Φ ((%l & %γ & -> & #Hmeta & #Hl_deques & #Hl_foreign & #Hl_waiters & #Hdeques_inv & #Hforeign_inv & #Hwaiters_inv & #Hinv) & (%_l & %_γ & %round & %n & %Heq & _Hmeta & #Hl_rounds & Hdeques_owner & #Hv_rounds & Hround)) HΦ". injection Heq as <-.
@@ -404,14 +386,14 @@ Section ws_hub_G.
     iInv "Hinv" as "(%vs & %vss & %vs_foreign & >%Hvs & >Hdeques_model & Hforeign_model & >Hmodel₂)".
     iApply (aacc_aupd_commit with "HΦ"); first solve_ndisj. iIntros "%_vs (%_l & %_γ & %Heq & _Hmeta & Hmodel₁)". injection Heq as <-.
     iDestruct (meta_agree with "Hmeta _Hmeta") as %<-. iClear "_Hmeta".
-    iDestruct (ws_hub_model_agree with "Hmodel₁ Hmodel₂") as %->.
+    iDestruct (ws_hub_1_model_agree with "Hmodel₁ Hmodel₂") as %->.
     iAaccIntro with "Hdeques_model".
     { iIntros "Hdeques_model !>".
       iSplitL "Hmodel₁"; first iSteps. iIntros "$ !>".
       iSteps.
     }
     iIntros "%vs' (%Hlookup & Hdeques_model)".
-    iMod (ws_hub_model_update ({[+v+]} ⊎ vs) with "Hmodel₁ Hmodel₂") as "(Hmodel₁ & Hmodel₂)".
+    iMod (ws_hub_1_model_update ({[+v+]} ⊎ vs) with "Hmodel₁ Hmodel₂") as "(Hmodel₁ & Hmodel₂)".
     iSplitL "Hmodel₁"; first iSteps. iIntros "!> HΦ !>".
     iSplitR "HΦ".
     { repeat iExists _. iFrame. iPureIntro.
@@ -422,18 +404,18 @@ Section ws_hub_G.
     }
     iIntros "Hdeques_owner Hround". clear.
 
-    wp_smart_apply ws_hub_notify_spec; iSteps.
+    wp_smart_apply ws_hub_1_notify_spec; iSteps.
   Qed.
 
-  Lemma ws_hub_push_foreign_spec t ι v :
+  Lemma ws_hub_1_push_foreign_spec t ι v :
     <<<
-      ws_hub_inv t ι
+      ws_hub_1_inv t ι
     | ∀∀ vs,
-      ws_hub_model t vs
+      ws_hub_1_model t vs
     >>>
-      ws_hub_push_foreign ws_deques t v @ ↑ι
+      ws_hub_1_push_foreign ws_deques t v @ ↑ι
     <<<
-      ws_hub_model t ({[+v+]} ⊎ vs)
+      ws_hub_1_model t ({[+v+]} ⊎ vs)
     | RET (); True
     >>>.
   Proof.
@@ -445,14 +427,14 @@ Section ws_hub_G.
     iInv "Hinv" as "(%vs & %vss & %vs_foreign & >%Hvs & Hdeques_model & >Hforeign_model & >Hmodel₂)".
     iApply (aacc_aupd_commit with "HΦ"); first solve_ndisj. iIntros "%_vs (%_l & %_γ & %Heq & _Hmeta & Hmodel₁)". injection Heq as <-.
     iDestruct (meta_agree with "Hmeta _Hmeta") as %<-. iClear "_Hmeta".
-    iDestruct (ws_hub_model_agree with "Hmodel₁ Hmodel₂") as %->.
+    iDestruct (ws_hub_1_model_agree with "Hmodel₁ Hmodel₂") as %->.
     iAaccIntro with "Hforeign_model".
     { iIntros "Hforeign_model !>".
       iSplitL "Hmodel₁"; first iSteps. iIntros "$ !>".
       iSteps.
     }
     iIntros "Hforeign_model".
-    iMod (ws_hub_model_update ({[+v+]} ⊎ vs) with "Hmodel₁ Hmodel₂") as "(Hmodel₁ & Hmodel₂)".
+    iMod (ws_hub_1_model_update ({[+v+]} ⊎ vs) with "Hmodel₁ Hmodel₂") as "(Hmodel₁ & Hmodel₂)".
     iSplitL "Hmodel₁"; first iSteps. iIntros "!> HΦ !>".
     iSplitR "HΦ".
     { repeat iExists _. iFrame. iPureIntro.
@@ -461,30 +443,30 @@ Section ws_hub_G.
     }
     iIntros "_". clear.
 
-    wp_smart_apply ws_hub_notify_spec; iSteps.
+    wp_smart_apply ws_hub_1_notify_spec; iSteps.
   Qed.
 
-  Lemma ws_hub_pop_spec t ι i :
+  Lemma ws_hub_1_pop_spec t ι i :
     (0 ≤ i)%Z →
     <<<
-      ws_hub_inv t ι ∗
-      ws_hub_owner t (Z.to_nat i)
+      ws_hub_1_inv t ι ∗
+      ws_hub_1_owner t (Z.to_nat i)
     | ∀∀ vs,
-      ws_hub_model t vs
+      ws_hub_1_model t vs
     >>>
-      ws_hub_pop ws_deques t #i @ ↑ι
+      ws_hub_1_pop ws_deques t #i @ ↑ι
     <<<
       ∃∃ o,
       match o with
       | None =>
-          ws_hub_model t vs
+          ws_hub_1_model t vs
       | Some v =>
           ∃ vs',
           ⌜vs = {[+v+]} ⊎ vs'⌝ ∗
-          ws_hub_model t vs'
+          ws_hub_1_model t vs'
       end
     | RET o;
-      ws_hub_owner t (Z.to_nat i)
+      ws_hub_1_owner t (Z.to_nat i)
     >>>.
   Proof.
     iIntros "%Hi !> %Φ ((%l & %γ & -> & #Hmeta & #Hl_deques & #Hl_foreign & #Hl_waiters & #Hdeques_inv & #Hforeign_inv & #Hwaiters_inv & #Hinv) & (%_l & %_γ & %round & %n & %Heq & _Hmeta & #Hl_rounds & Hdeques_owner & #Hv_rounds & Hround)) HΦ". injection Heq as <-.
@@ -496,7 +478,7 @@ Section ws_hub_G.
     iInv "Hinv" as "(%vs & %vss & %vs_foreign & >%Hvs & >Hdeques_model & Hforeign_model & >Hmodel₂)".
     iApply (aacc_aupd_commit with "HΦ"); first solve_ndisj. iIntros "%_vs (%_l & %_γ & %Heq & _Hmeta & Hmodel₁)". injection Heq as <-.
     iDestruct (meta_agree with "Hmeta _Hmeta") as %<-. iClear "_Hmeta".
-    iDestruct (ws_hub_model_agree with "Hmodel₁ Hmodel₂") as %->.
+    iDestruct (ws_hub_1_model_agree with "Hmodel₁ Hmodel₂") as %->.
     iAaccIntro with "Hdeques_model".
     { iIntros "Hdeques_model !>".
       iSplitL "Hmodel₁"; iSteps.
@@ -505,7 +487,7 @@ Section ws_hub_G.
 
     - iDestruct "Hdeques_model" as "(%ws & %Hlookup & Hdeques_model)".
       set vs' := vs ∖ {[+v+]}.
-      iMod (ws_hub_model_update vs' with "Hmodel₁ Hmodel₂") as "(Hmodel₁ & Hmodel₂)".
+      iMod (ws_hub_1_model_update vs' with "Hmodel₁ Hmodel₂") as "(Hmodel₁ & Hmodel₂)".
       iExists (Some v).
       iSplitL "Hmodel₁".
       { iExists vs'. iSteps. iPureIntro.
@@ -530,22 +512,22 @@ Section ws_hub_G.
       iSplitL "Hmodel₁"; iSteps.
   Qed.
 
-  #[local] Lemma ws_hub_pop_foreign_spec t ι :
+  #[local] Lemma ws_hub_1_pop_foreign_spec t ι :
     <<<
-      ws_hub_inv t ι
+      ws_hub_1_inv t ι
     | ∀∀ vs,
-      ws_hub_model t vs
+      ws_hub_1_model t vs
     >>>
-      ws_hub_pop_foreign t @ ↑ι
+      ws_hub_1_pop_foreign t @ ↑ι
     <<<
       ∃∃ o,
       match o with
       | None =>
-          ws_hub_model t vs
+          ws_hub_1_model t vs
       | Some v =>
           ∃ vs',
           ⌜vs = {[+v+]} ⊎ vs'⌝ ∗
-          ws_hub_model t vs'
+          ws_hub_1_model t vs'
       end
     | RET o; True
     >>>.
@@ -558,7 +540,7 @@ Section ws_hub_G.
     iInv "Hinv" as "(%vs & %vss & %vs_foreign & >%Hvs & Hdeques_model & >Hforeign_model & >Hmodel₂)".
     iApply (aacc_aupd_commit with "HΦ"); first solve_ndisj. iIntros "%_vs (%_l & %_γ & %Heq & _Hmeta & Hmodel₁)". injection Heq as <-.
     iDestruct (meta_agree with "Hmeta _Hmeta") as %<-. iClear "_Hmeta".
-    iDestruct (ws_hub_model_agree with "Hmodel₁ Hmodel₂") as %->.
+    iDestruct (ws_hub_1_model_agree with "Hmodel₁ Hmodel₂") as %->.
     iAaccIntro with "Hforeign_model".
     { iIntros "Hforeign_model !>".
       iSplitL "Hmodel₁"; iSteps.
@@ -570,7 +552,7 @@ Section ws_hub_G.
       iSplitL "Hmodel₁"; iSteps.
 
     - set vs' := vs ∖ {[+v+]}.
-      iMod (ws_hub_model_update vs' with "Hmodel₁ Hmodel₂") as "(Hmodel₁ & Hmodel₂)".
+      iMod (ws_hub_1_model_update vs' with "Hmodel₁ Hmodel₂") as "(Hmodel₁ & Hmodel₂)".
       iExists (Some v).
       iSplitL "Hmodel₁".
       { iExists vs'. iSteps. iPureIntro.
@@ -587,27 +569,27 @@ Section ws_hub_G.
       iSteps.
   Qed.
 
-  #[local] Lemma ws_hub_try_steal_once_spec t ι i :
+  #[local] Lemma ws_hub_1_try_steal_once_spec t ι i :
     (0 ≤ i)%Z →
     <<<
-      ws_hub_inv t ι ∗
-      ws_hub_owner t (Z.to_nat i)
+      ws_hub_1_inv t ι ∗
+      ws_hub_1_owner t (Z.to_nat i)
     | ∀∀ vs,
-      ws_hub_model t vs
+      ws_hub_1_model t vs
     >>>
-      ws_hub_try_steal_once ws_deques t #i @ ↑ι
+      ws_hub_1_try_steal_once ws_deques t #i @ ↑ι
     <<<
       ∃∃ o,
       match o with
       | None =>
-          ws_hub_model t vs
+          ws_hub_1_model t vs
       | Some v =>
           ∃ vs',
           ⌜vs = {[+v+]} ⊎ vs'⌝ ∗
-          ws_hub_model t vs'
+          ws_hub_1_model t vs'
       end
     | RET o;
-      ws_hub_owner t (Z.to_nat i)
+      ws_hub_1_owner t (Z.to_nat i)
     >>>.
   Proof.
     iIntros "%Hi !> %Φ ((%l & %γ & -> & #Hmeta & #Hl_deques & #Hl_foreign & #Hl_waiters & #Hdeques_inv & #Hforeign_inv & #Hwaiters_inv & #Hinv) & (%_l & %_γ & %round & %n & %Heq & _Hmeta & #Hl_rounds & Hdeques_owner & #Hv_rounds & Hround)) HΦ". injection Heq as <-.
@@ -623,7 +605,7 @@ Section ws_hub_G.
     iInv "Hinv" as "(%vs & %vss & %vs_foreign & >%Hvs & >Hdeques_model & Hforeign_model & >Hmodel₂)".
     iApply (aacc_aupd_commit with "HΦ"); first solve_ndisj. iIntros "%_vs (%_l & %_γ & %Heq & _Hmeta & Hmodel₁)". injection Heq as <-.
     iDestruct (meta_agree with "Hmeta _Hmeta") as %<-. iClear "_Hmeta".
-    iDestruct (ws_hub_model_agree with "Hmodel₁ Hmodel₂") as %->.
+    iDestruct (ws_hub_1_model_agree with "Hmodel₁ Hmodel₂") as %->.
     iAaccIntro with "Hdeques_model".
     { iIntros "Hdeques_model !>".
       iSplitL "Hmodel₁"; iSteps.
@@ -632,7 +614,7 @@ Section ws_hub_G.
 
     - iDestruct "Hdeques_model" as "(%j & %ws & %Hj & %Hlookup & Hdeques_model)".
       set vs' := vs ∖ {[+v+]}.
-      iMod (ws_hub_model_update vs' with "Hmodel₁ Hmodel₂") as "(Hmodel₁ & Hmodel₂)".
+      iMod (ws_hub_1_model_update vs' with "Hmodel₁ Hmodel₂") as "(Hmodel₁ & Hmodel₂)".
       iExists (Some v).
       iSplitL "Hmodel₁".
       { iExists vs'. iSteps. iPureIntro.
@@ -655,28 +637,28 @@ Section ws_hub_G.
       iSplitL "Hmodel₁"; iSteps.
   Qed.
 
-  #[local] Lemma ws_hub_try_steal_aux_spec yield t ι i max_round :
+  #[local] Lemma ws_hub_1_try_steal_aux_spec yield t ι i max_round :
     (0 ≤ i)%Z →
     (0 ≤ max_round)%Z →
     <<<
-      ws_hub_inv t ι ∗
-      ws_hub_owner t (Z.to_nat i)
+      ws_hub_1_inv t ι ∗
+      ws_hub_1_owner t (Z.to_nat i)
     | ∀∀ vs,
-      ws_hub_model t vs
+      ws_hub_1_model t vs
     >>>
-      ws_hub_try_steal_aux ws_deques yield t #i #max_round @ ↑ι
+      ws_hub_1_try_steal_aux ws_deques yield t #i #max_round @ ↑ι
     <<<
       ∃∃ o,
       match o with
       | None =>
-          ws_hub_model t vs
+          ws_hub_1_model t vs
       | Some v =>
           ∃ vs',
           ⌜vs = {[+v+]} ⊎ vs'⌝ ∗
-          ws_hub_model t vs'
+          ws_hub_1_model t vs'
       end
     | RET o;
-      ws_hub_owner t (Z.to_nat i)
+      ws_hub_1_owner t (Z.to_nat i)
     >>>.
   Proof.
     intros Hi.
@@ -692,7 +674,7 @@ Section ws_hub_G.
       iApply ("HΦ" $! None with "Hmodel").
       iSteps.
 
-    - awp_apply ws_hub_pop_foreign_spec without "Hdeques_owner Hround"; first iSteps.
+    - awp_apply ws_hub_1_pop_foreign_spec without "Hdeques_owner Hround"; first iSteps.
       iApply (aacc_aupd with "HΦ"); first done. iIntros "%vs Hmodel".
       iAaccIntro with "Hmodel"; first iSteps. iIntros ([v |]) "Hmodel !>".
 
@@ -702,7 +684,7 @@ Section ws_hub_G.
       + iLeft. iFrame.
         iIntros "HΦ !> _ (Hdeques_owner & Hround)". clear- Hi Hmax_round Hcase.
 
-        awp_smart_apply (ws_hub_try_steal_once_spec with "[Hdeques_owner Hround]"); [done | iSteps |].
+        awp_smart_apply (ws_hub_1_try_steal_once_spec with "[Hdeques_owner Hround]"); [done | iSteps |].
         iApply (aacc_aupd with "HΦ"); first done. iIntros "%vs Hmodel".
         iAaccIntro with "Hmodel"; first iSteps. iIntros ([v |]) "Hmodel !>".
 
@@ -721,36 +703,36 @@ Section ws_hub_G.
           { destruct yield; iSteps. }
           wp_smart_apply ("HLöb" with "[] [$Howner] HΦ"); iSteps.
   Qed.
-  Lemma ws_hub_try_steal_spec t ι i max_round_noyield max_round_yield :
+  Lemma ws_hub_1_try_steal_spec t ι i max_round_noyield max_round_yield :
     (0 ≤ i)%Z →
     (0 ≤ max_round_noyield)%Z →
     (0 ≤ max_round_yield)%Z →
     <<<
-      ws_hub_inv t ι ∗
-      ws_hub_owner t (Z.to_nat i)
+      ws_hub_1_inv t ι ∗
+      ws_hub_1_owner t (Z.to_nat i)
     | ∀∀ vs,
-      ws_hub_model t vs
+      ws_hub_1_model t vs
     >>>
-      ws_hub_try_steal ws_deques t #i (#max_round_noyield, #max_round_yield)%V @ ↑ι
+      ws_hub_1_try_steal ws_deques t #i (#max_round_noyield, #max_round_yield)%V @ ↑ι
     <<<
       ∃∃ o,
       match o with
       | None =>
-          ws_hub_model t vs
+          ws_hub_1_model t vs
       | Some v =>
           ∃ vs',
           ⌜vs = {[+v+]} ⊎ vs'⌝ ∗
-          ws_hub_model t vs'
+          ws_hub_1_model t vs'
       end
     | RET o;
-      ws_hub_owner t (Z.to_nat i)
+      ws_hub_1_owner t (Z.to_nat i)
     >>>.
   Proof.
     iIntros "%Hi %Hmax_round_noyield %Hmax_round_yield !> %Φ (#Hinv & Howner) HΦ".
 
     wp_rec.
 
-    awp_smart_apply (ws_hub_try_steal_aux_spec with "[$Hinv $Howner]"); [done.. |].
+    awp_smart_apply (ws_hub_1_try_steal_aux_spec with "[$Hinv $Howner]"); [done.. |].
     iApply (aacc_aupd with "HΦ"); first done. iIntros "%vs Hmodel".
     iAaccIntro with "Hmodel"; first iSteps. iIntros ([v |]) "Hmodel !>".
 
@@ -763,71 +745,26 @@ Section ws_hub_G.
     - iLeft. iFrame.
       iIntros "HΦ !> Howner". clear- Hi Hmax_round_yield.
 
-      wp_smart_apply (ws_hub_try_steal_aux_spec with "[$Hinv $Howner] HΦ"); done.
+      wp_smart_apply (ws_hub_1_try_steal_aux_spec with "[$Hinv $Howner] HΦ"); done.
   Qed.
 
-  Lemma ws_hub_pop_try_steal_spec t ι i max_round_noyield max_round_yield :
+  Lemma ws_hub_1_steal_spec t ι i max_round_noyield max_round_yield :
     (0 ≤ i)%Z →
     (0 ≤ max_round_noyield)%Z →
     (0 ≤ max_round_yield)%Z →
     <<<
-      ws_hub_inv t ι ∗
-      ws_hub_owner t (Z.to_nat i)
+      ws_hub_1_inv t ι ∗
+      ws_hub_1_owner t (Z.to_nat i)
     | ∀∀ vs,
-      ws_hub_model t vs
+      ws_hub_1_model t vs
     >>>
-      ws_hub_pop_try_steal ws_deques t #i (#max_round_noyield, #max_round_yield)%V @ ↑ι
-    <<<
-      ∃∃ o,
-      match o with
-      | None =>
-          ws_hub_model t vs
-      | Some v =>
-          ∃ vs',
-          ⌜vs = {[+v+]} ⊎ vs'⌝ ∗
-          ws_hub_model t vs'
-      end
-    | RET o;
-      ws_hub_owner t (Z.to_nat i)
-    >>>.
-  Proof.
-    iIntros "%Hi %Hmax_round_noyield %Hmax_round_yield !> %Φ (#Hinv & Howner) HΦ".
-
-    wp_rec.
-
-    awp_smart_apply (ws_hub_pop_spec with "[$Hinv $Howner]"); [done.. |].
-    iApply (aacc_aupd with "HΦ"); first done. iIntros "%vs Hmodel".
-    iAaccIntro with "Hmodel"; first iSteps. iIntros ([v |]) "Hmodel !>".
-
-    - iRight. iExists (Some v). iFrame.
-      iIntros "HΦ !> Howner". clear.
-
-      iSpecialize ("HΦ" with "Howner").
-      iSteps.
-
-    - iLeft. iFrame.
-      iIntros "HΦ !> Howner". clear- Hi Hmax_round_noyield Hmax_round_yield.
-
-      wp_smart_apply (ws_hub_try_steal_spec with "[$Hinv $Howner] HΦ"); done.
-  Qed.
-
-  Lemma ws_hub_steal_spec t ι i max_round_noyield max_round_yield :
-    (0 ≤ i)%Z →
-    (0 ≤ max_round_noyield)%Z →
-    (0 ≤ max_round_yield)%Z →
-    <<<
-      ws_hub_inv t ι ∗
-      ws_hub_owner t (Z.to_nat i)
-    | ∀∀ vs,
-      ws_hub_model t vs
-    >>>
-      ws_hub_steal ws_deques t #i (#max_round_noyield, #max_round_yield)%V @ ↑ι
+      ws_hub_1_steal ws_deques t #i (#max_round_noyield, #max_round_yield)%V @ ↑ι
     <<<
       ∃∃ v vs',
       ⌜vs = {[+v+]} ⊎ vs'⌝ ∗
-      ws_hub_model t vs'
+      ws_hub_1_model t vs'
     | RET v;
-      ws_hub_owner t (Z.to_nat i)
+      ws_hub_1_owner t (Z.to_nat i)
     >>>.
   Proof.
     iIntros "%Hi %Hmax_round_noyield %Hmax_round_yield !> %Φ (#Hinv & Howner) HΦ".
@@ -836,7 +773,7 @@ Section ws_hub_G.
 
     wp_rec.
 
-    awp_smart_apply (ws_hub_try_steal_spec with "[$Hinv $Howner]"); [done.. |].
+    awp_smart_apply (ws_hub_1_try_steal_spec with "[$Hinv $Howner]"); [done.. |].
     iApply (aacc_aupd with "HΦ"); first done. iIntros "%vs Hmodel".
     iAaccIntro with "Hmodel"; first iSteps. iIntros ([v |]) "Hmodel !>".
 
@@ -851,7 +788,7 @@ Section ws_hub_G.
       wp_load.
       wp_smart_apply (waiters_prepare_wait_spec with "Hwaiters_inv") as (waiter) "Hwaiter".
 
-      awp_smart_apply (ws_hub_try_steal_once_spec with "[$Howner]") without "Hwaiter"; [done.. | iSteps |].
+      awp_smart_apply (ws_hub_1_try_steal_once_spec with "[$Howner]") without "Hwaiter"; [done.. | iSteps |].
       iApply (aacc_aupd with "HΦ"); first done. iIntros "%vs Hmodel".
       iAaccIntro with "Hmodel"; first iSteps. iIntros ([v |]) "Hmodel !>".
 
@@ -870,56 +807,24 @@ Section ws_hub_G.
         wp_smart_apply ("HLöb" with "Howner HΦ").
   Qed.
 
-  Lemma ws_hub_pop_steal_spec t ι i max_round_noyield max_round_yield :
-    (0 ≤ i)%Z →
-    (0 ≤ max_round_noyield)%Z →
-    (0 ≤ max_round_yield)%Z →
-    <<<
-      ws_hub_inv t ι ∗
-      ws_hub_owner t (Z.to_nat i)
-    | ∀∀ vs,
-      ws_hub_model t vs
-    >>>
-      ws_hub_pop_steal ws_deques t #i (#max_round_noyield, #max_round_yield)%V @ ↑ι
-    <<<
-      ∃∃ v vs',
-      ⌜vs = {[+v+]} ⊎ vs'⌝ ∗
-      ws_hub_model t vs'
-    | RET v;
-      ws_hub_owner t (Z.to_nat i)
-    >>>.
-  Proof.
-    iIntros "%Hi %Hmax_round_noyield %Hmax_round_yield !> %Φ (#Hinv & Howner) HΦ".
+  Definition ws_hub_1 :=
+    Build_ws_hub
+      ws_hub_1_owner_exclusive
+      ws_hub_1_create_spec
+      ws_hub_1_push_spec
+      ws_hub_1_push_foreign_spec
+      ws_hub_1_pop_spec
+      ws_hub_1_try_steal_spec
+      ws_hub_1_steal_spec.
+End ws_hub_1_G.
 
-    wp_rec.
+#[global] Opaque ws_hub_1_create.
+#[global] Opaque ws_hub_1_push.
+#[global] Opaque ws_hub_1_push_foreign.
+#[global] Opaque ws_hub_1_pop.
+#[global] Opaque ws_hub_1_try_steal.
+#[global] Opaque ws_hub_1_steal.
 
-    awp_smart_apply (ws_hub_pop_spec with "[$Hinv $Howner]"); [done.. |].
-    iApply (aacc_aupd with "HΦ"); first done. iIntros "%vs Hmodel".
-    iAaccIntro with "Hmodel"; first iSteps. iIntros ([v |]) "Hmodel !>".
-
-    - iDestruct "Hmodel" as "(%vs' & -> & Hmodel)".
-      iRight. iExists v, vs'. iFrame. iStep.
-      iIntros "HΦ !> Howner". clear.
-
-      iSpecialize ("HΦ" with "Howner").
-      iSteps.
-
-    - iLeft. iFrame.
-      iIntros "HΦ !> Howner". clear- Hi Hmax_round_noyield Hmax_round_yield.
-
-      wp_smart_apply (ws_hub_steal_spec with "[$Hinv $Howner] HΦ"); done.
-  Qed.
-End ws_hub_G.
-
-#[global] Opaque ws_hub_create.
-#[global] Opaque ws_hub_push.
-#[global] Opaque ws_hub_push_foreign.
-#[global] Opaque ws_hub_pop.
-#[global] Opaque ws_hub_try_steal.
-#[global] Opaque ws_hub_pop_try_steal.
-#[global] Opaque ws_hub_steal.
-#[global] Opaque ws_hub_pop_steal.
-
-#[global] Opaque ws_hub_inv.
-#[global] Opaque ws_hub_model.
-#[global] Opaque ws_hub_owner.
+#[global] Opaque ws_hub_1_inv.
+#[global] Opaque ws_hub_1_model.
+#[global] Opaque ws_hub_1_owner.
