theories/parabstr/ws_hub_2.v
@@ -21,7 +21,7 @@ From zebre.std Require Import
 From zebre.saturn Require Import
   mpmc_queue_1.
 From zebre.parabstr Require Export
-  base.
+  ws_hub.
 From zebre.parabstr Require Import
   ws_deques
   waiters.
@@ -63,7 +63,7 @@ Section ws_deques.
   Context `{zebre_G : !ZebreG Σ}.
   Context (ws_deques : ws_deques Σ).
 
-  Definition ws_hub_create : val :=
+  Definition ws_hub_2_create : val :=
     λ: "sz",
       { ws_deques.(ws_deques_create) "sz";
         mpmc_queue_create ();
@@ -73,293 +73,275 @@ Section ws_deques.
         #0
       }.
 
-  #[local] Definition ws_hub_num_worker : val :=
+  #[local] Definition ws_hub_2_num_worker : val :=
     λ: "t",
       "t".{num_worker}.
-  #[local] Definition ws_hub_num_thief : val :=
+  #[local] Definition ws_hub_2_num_thief : val :=
     λ: "t",
       "t".{num_thief}.
 
-  #[local] Definition ws_hub_incr_num_worker : val :=
+  #[local] Definition ws_hub_2_incr_num_worker : val :=
     λ: "t",
       Faa "t".[num_worker] #1.
-  #[local] Definition ws_hub_decr_num_worker : val :=
+  #[local] Definition ws_hub_2_decr_num_worker : val :=
     λ: "t",
       Faa "t".[num_worker] #-1.
 
-  #[local] Definition ws_hub_incr_num_thief : val :=
+  #[local] Definition ws_hub_2_incr_num_thief : val :=
     λ: "t",
       Faa "t".[num_thief] #1.
-  #[local] Definition ws_hub_decr_num_thief : val :=
+  #[local] Definition ws_hub_2_decr_num_thief : val :=
     λ: "t",
       Faa "t".[num_thief] #-1.
 
-  #[local] Definition ws_hub_notify : val :=
+  #[local] Definition ws_hub_2_notify : val :=
     λ: "t",
       waiters_notify "t".{waiters}.
 
-  Definition ws_hub_push : val :=
+  Definition ws_hub_2_push : val :=
     λ: "t" "i" "v",
       ws_deques.(ws_deques_push) "t".{deques} "i" "v".
 
   #[using="ws_deques"]
-  Definition ws_hub_push_foreign : val :=
+  Definition ws_hub_2_push_foreign : val :=
     λ: "t" "v",
       mpmc_queue_push "t".{foreign} "v".
 
-  Definition ws_hub_pop : val :=
+  Definition ws_hub_2_pop : val :=
     λ: "t" "i",
       ws_deques.(ws_deques_pop) "t".{deques} "i".
 
-  #[local] Definition ws_hub_pop_foreign : val :=
+  #[local] Definition ws_hub_2_pop_foreign : val :=
     λ: "t",
       mpmc_queue_pop "t".{foreign}.
 
-  #[local] Definition ws_hub_try_steal_once : val :=
+  #[local] Definition ws_hub_2_try_steal_once : val :=
     λ: "t" "i",
       let: "round" := array_unsafe_get "t".{rounds} "i" in
       random_round_reset "round" ;;
       ws_deques_steal_as ws_deques "t".{deques} "i" "round".
 
-  #[local] Definition ws_hub_try_steal_aux yield : val :=
-    rec: "ws_hub_try_steal_aux" "t" "i" "max_round" :=
+  #[local] Definition ws_hub_2_try_steal_aux yield : val :=
+    rec: "ws_hub_2_try_steal_aux" "t" "i" "max_round" :=
       if: "max_round" ≤ #0 then (
         §None
       ) else (
-        match: ws_hub_pop_foreign "t" with
+        match: ws_hub_2_pop_foreign "t" with
         | Some <> as "res" =>
             "res"
         | None =>
-            match: ws_hub_try_steal_once "t" "i" with
+            match: ws_hub_2_try_steal_once "t" "i" with
             | Some <> as "res" =>
                 "res"
             | None =>
                 (if yield then Yield else ()) ;;
-                "ws_hub_try_steal_aux" "t" "i" ("max_round" - #1)
+                "ws_hub_2_try_steal_aux" "t" "i" ("max_round" - #1)
             end
         end
       ).
-  Definition ws_hub_try_steal : val :=
+  Definition ws_hub_2_try_steal : val :=
     λ: "t" "i" "max_round",
-      match: ws_hub_try_steal_aux false "t" "i" "max_round".<0> with
+      match: ws_hub_2_try_steal_aux false "t" "i" "max_round".<0> with
       | Some <> as "res" =>
           "res"
       | None =>
-          ws_hub_try_steal_aux true "t" "i" "max_round".<1>
+          ws_hub_2_try_steal_aux true "t" "i" "max_round".<1>
       end.
 
-  Definition ws_hub_pop_try_steal : val :=
-    λ: "t" "i" "max_round",
-      match: ws_hub_pop "t" "i" with
-      | Some <> as "res" =>
-          "res"
-      | None =>
-          ws_hub_try_steal "t" "i" "max_round"
-      end.
-
-  #[local] Definition ws_hub_steal_init : val :=
+  #[local] Definition ws_hub_2_steal_init : val :=
     λ: "t",
-      ws_hub_incr_num_thief "t" ;;
+      ws_hub_2_incr_num_thief "t" ;;
       ().
-  #[local] Definition ws_hub_steal_2 : val :=
-    rec: "ws_hub_steal_2" "t" "i" "max_round" :=
-      match: ws_hub_try_steal "t" "i" "max_round" with
+  #[local] Definition ws_hub_2_steal_2 : val :=
+    rec: "ws_hub_2_steal_2" "t" "i" "max_round" :=
+      match: ws_hub_2_try_steal "t" "i" "max_round" with
       | Some "v" =>
           "v"
       | None =>
           let: "waiters" := "t".{waiters} in
           let: "waiter" := waiters_prepare_wait "waiters" in
           if: mpmc_queue_is_empty "t".{foreign} then (
-            if: ws_hub_decr_num_thief "t" = #1 and #0 < ws_hub_num_worker "t" then (
+            if: ws_hub_2_decr_num_thief "t" = #1 and #0 < ws_hub_2_num_worker "t" then (
               waiters_cancel_wait "waiters" "waiter"
             ) else (
               waiters_commit_wait "waiters" "waiter"
             ) ;;
-            ws_hub_steal_init "t" ;;
-            "ws_hub_steal_2" "t" "i" "max_round"
+            ws_hub_2_steal_init "t" ;;
+            "ws_hub_2_steal_2" "t" "i" "max_round"
           ) else (
             waiters_cancel_wait "waiters" "waiter" ;;
-            match: ws_hub_pop_foreign "t" with
+            match: ws_hub_2_pop_foreign "t" with
             | Some "v" =>
                 "v"
             | None =>
-                "ws_hub_steal_2" "t" "i" "max_round"
+                "ws_hub_2_steal_2" "t" "i" "max_round"
             end
           )
       end.
-  #[local] Definition ws_hub_steal_1 : val :=
+  #[local] Definition ws_hub_2_steal_1 : val :=
     λ: "t" "i" "max_round",
-      ws_hub_steal_init "t" ;;
-      let: "v" := ws_hub_steal_2 "t" "i" "max_round" in
-      if: ws_hub_decr_num_thief "t" = #1 then (
-        ws_hub_notify "t"
+      ws_hub_2_steal_init "t" ;;
+      let: "v" := ws_hub_2_steal_2 "t" "i" "max_round" in
+      if: ws_hub_2_decr_num_thief "t" = #1 then (
+        ws_hub_2_notify "t"
       ) else (
         ()
       ) ;;
       "v".
-  Definition ws_hub_steal : val :=
+  Definition ws_hub_2_steal : val :=
     λ: "t" "i" "max_round",
-      ws_hub_decr_num_worker "t" ;;
-      let: "v" := ws_hub_steal_1 "t" "i" "max_round" in
-      if: ws_hub_incr_num_worker "t" = #0 and ws_hub_num_thief "t" = #0 then (
-        ws_hub_notify "t"
+      ws_hub_2_decr_num_worker "t" ;;
+      let: "v" := ws_hub_2_steal_1 "t" "i" "max_round" in
+      if: ws_hub_2_incr_num_worker "t" = #0 and ws_hub_2_num_thief "t" = #0 then (
+        ws_hub_2_notify "t"
       ) else (
         ()
       ) ;;
       "v".
-
-  Definition ws_hub_pop_steal : val :=
-    λ: "t" "i" "max_round",
-      match: ws_hub_pop "t" "i" with
-      | Some "v" =>
-          "v"
-      | None =>
-          ws_hub_steal "t" "i" "max_round"
-      end.
 End ws_deques.
 
-Class WsHubG Σ `{zebre_G : !ZebreG Σ} := {
-  #[local] ws_hub_G_queue_G :: MpmcQueueG Σ ;
-  #[local] ws_hub_G_waiters_G :: WaitersG Σ ;
-  #[local] ws_hub_G_model_G :: TwinsG Σ (leibnizO (gmultiset val)) ;
+Class WsHub2G Σ `{zebre_G : !ZebreG Σ} := {
+  #[local] ws_hub_2_G_queue_G :: MpmcQueueG Σ ;
+  #[local] ws_hub_2_G_waiters_G :: WaitersG Σ ;
+  #[local] ws_hub_2_G_model_G :: TwinsG Σ (leibnizO (gmultiset val)) ;
 }.
 
-Definition ws_hub_Σ := #[
+Definition ws_hub_2_Σ := #[
   mpmc_queue_Σ ;
   waiters_Σ ;
   twins_Σ (leibnizO (gmultiset val))
 ].
-#[global] Instance subG_ws_hub_Σ Σ `{zebre_G : !ZebreG Σ} :
-  subG ws_hub_Σ Σ →
-  WsHubG Σ.
+#[global] Instance subG_ws_hub_2_Σ Σ `{zebre_G : !ZebreG Σ} :
+  subG ws_hub_2_Σ Σ →
+  WsHub2G Σ.
 Proof.
   solve_inG.
 Qed.
 
-Section ws_hub_G.
-  Context `{ws_hub_G : WsHubG Σ}.
+Section ws_hub_2_G.
+  Context `{ws_hub_2_G : WsHub2G Σ}.
   Context (ws_deques : ws_deques Σ).
 
-  Record ws_hub_meta := {
-    ws_hub_meta_size : nat ;
-    ws_hub_meta_deques : val ;
-    ws_hub_meta_foreign : val ;
-    ws_hub_meta_rounds : val ;
-    ws_hub_meta_waiters : val ;
-    ws_hub_meta_model : gname ;
+  Record ws_hub_2_meta := {
+    ws_hub_2_meta_size : nat ;
+    ws_hub_2_meta_deques : val ;
+    ws_hub_2_meta_foreign : val ;
+    ws_hub_2_meta_rounds : val ;
+    ws_hub_2_meta_waiters : val ;
+    ws_hub_2_meta_model : gname ;
   }.
-  Implicit Types γ : ws_hub_meta.
+  Implicit Types γ : ws_hub_2_meta.
 
-  #[local] Instance ws_hub_meta_eq_dec :
-    EqDecision ws_hub_meta.
+  #[local] Instance ws_hub_2_meta_eq_dec :
+    EqDecision ws_hub_2_meta.
   Proof.
     solve_decision.
   Qed.
-  #[local] Instance ws_hub_meta_countable :
-    Countable ws_hub_meta.
+  #[local] Instance ws_hub_2_meta_countable :
+    Countable ws_hub_2_meta.
   Proof.
     pose encode γ := (
-      γ.(ws_hub_meta_size),
-      γ.(ws_hub_meta_deques),
-      γ.(ws_hub_meta_foreign),
-      γ.(ws_hub_meta_rounds),
-      γ.(ws_hub_meta_waiters),
-      γ.(ws_hub_meta_model)
+      γ.(ws_hub_2_meta_size),
+      γ.(ws_hub_2_meta_deques),
+      γ.(ws_hub_2_meta_foreign),
+      γ.(ws_hub_2_meta_rounds),
+      γ.(ws_hub_2_meta_waiters),
+      γ.(ws_hub_2_meta_model)
     ).
     pose decode := λ '(γ_size, γ_deques, γ_foreign, γ_rounds, γ_waiters, γ_model), {|
-      ws_hub_meta_size := γ_size ;
-      ws_hub_meta_deques := γ_deques ;
-      ws_hub_meta_foreign := γ_foreign ;
-      ws_hub_meta_rounds := γ_rounds ;
-      ws_hub_meta_waiters := γ_waiters ;
-      ws_hub_meta_model := γ_model ;
+      ws_hub_2_meta_size := γ_size ;
+      ws_hub_2_meta_deques := γ_deques ;
+      ws_hub_2_meta_foreign := γ_foreign ;
+      ws_hub_2_meta_rounds := γ_rounds ;
+      ws_hub_2_meta_waiters := γ_waiters ;
+      ws_hub_2_meta_model := γ_model ;
     |}.
     refine (inj_countable' encode decode _). intros []. done.
   Qed.
 
-  #[local] Definition ws_hub_model₁' γ_model vs :=
+  #[local] Definition ws_hub_2_model₁' γ_model vs :=
     twins_twin1 γ_model (DfracOwn 1) vs.
-  #[local] Definition ws_hub_model₁ γ vs :=
-    ws_hub_model₁' γ.(ws_hub_meta_model) vs.
-  #[local] Definition ws_hub_model₂' γ_model vs :=
+  #[local] Definition ws_hub_2_model₁ γ vs :=
+    ws_hub_2_model₁' γ.(ws_hub_2_meta_model) vs.
+  #[local] Definition ws_hub_2_model₂' γ_model vs :=
     twins_twin2 γ_model vs.
-  #[local] Definition ws_hub_model₂ γ vs :=
-    ws_hub_model₂' γ.(ws_hub_meta_model) vs.
+  #[local] Definition ws_hub_2_model₂ γ vs :=
+    ws_hub_2_model₂' γ.(ws_hub_2_meta_model) vs.
 
-  #[local] Definition ws_hub_inv_inner l γ : iProp Σ :=
+  #[local] Definition ws_hub_2_inv_inner l γ : iProp Σ :=
     ∃ vs vss vs_foreign num_worker num_thief,
     ⌜vs = foldr (λ vs_deques vs, list_to_set_disj vs_deques ⊎ vs) (list_to_set_disj vs_foreign) vss⌝ ∗
     l.[num_worker] ↦ #num_worker ∗
     l.[num_thief] ↦ #num_thief ∗
-    ws_deques.(ws_deques_model) γ.(ws_hub_meta_deques) vss ∗
-    mpmc_queue_model γ.(ws_hub_meta_foreign) vs_foreign ∗
-    ws_hub_model₂ γ vs.
-  Definition ws_hub_inv t ι : iProp Σ :=
+    ws_deques.(ws_deques_model) γ.(ws_hub_2_meta_deques) vss ∗
+    mpmc_queue_model γ.(ws_hub_2_meta_foreign) vs_foreign ∗
+    ws_hub_2_model₂ γ vs.
+  Definition ws_hub_2_inv t ι : iProp Σ :=
     ∃ l γ,
     ⌜t = #l⌝ ∗
     meta l nroot γ ∗
-    l.[deques] ↦□ γ.(ws_hub_meta_deques) ∗
-    l.[foreign] ↦□ γ.(ws_hub_meta_foreign) ∗
-    l.[waiters] ↦□ γ.(ws_hub_meta_waiters) ∗
-    ws_deques.(ws_deques_inv) γ.(ws_hub_meta_deques) (ι.@"deques") γ.(ws_hub_meta_size) ∗
-    mpmc_queue_inv γ.(ws_hub_meta_foreign) (ι.@"foreign") ∗
-    waiters_inv γ.(ws_hub_meta_waiters) ∗
-    inv (ι.@"inv") (ws_hub_inv_inner l γ).
+    l.[deques] ↦□ γ.(ws_hub_2_meta_deques) ∗
+    l.[foreign] ↦□ γ.(ws_hub_2_meta_foreign) ∗
+    l.[waiters] ↦□ γ.(ws_hub_2_meta_waiters) ∗
+    ws_deques.(ws_deques_inv) γ.(ws_hub_2_meta_deques) (ι.@"deques") γ.(ws_hub_2_meta_size) ∗
+    mpmc_queue_inv γ.(ws_hub_2_meta_foreign) (ι.@"foreign") ∗
+    waiters_inv γ.(ws_hub_2_meta_waiters) ∗
+    inv (ι.@"inv") (ws_hub_2_inv_inner l γ).
 
   #[using="ws_deques"]
-  Definition ws_hub_model t vs : iProp Σ :=
+  Definition ws_hub_2_model t vs : iProp Σ :=
     ∃ l γ,
     ⌜t = #l⌝ ∗
     meta l nroot γ ∗
-    ws_hub_model₁ γ vs.
+    ws_hub_2_model₁ γ vs.
 
-  Definition ws_hub_owner t i : iProp Σ :=
+  Definition ws_hub_2_owner t i : iProp Σ :=
     ∃ l γ round n,
     ⌜t = #l⌝ ∗
     meta l nroot γ ∗
-    l.[rounds] ↦□ γ.(ws_hub_meta_rounds) ∗
-    ws_deques.(ws_deques_owner) γ.(ws_hub_meta_deques) i ∗
-    array_slice γ.(ws_hub_meta_rounds) γ.(ws_hub_meta_size) i DfracDiscarded [round] ∗
-    random_round_model' round (γ.(ws_hub_meta_size) - 1) n.
+    l.[rounds] ↦□ γ.(ws_hub_2_meta_rounds) ∗
+    ws_deques.(ws_deques_owner) γ.(ws_hub_2_meta_deques) i ∗
+    array_slice γ.(ws_hub_2_meta_rounds) γ.(ws_hub_2_meta_size) i DfracDiscarded [round] ∗
+    random_round_model' round (γ.(ws_hub_2_meta_size) - 1) n.
 
-  #[global] Instance ws_hub_model_timeless t vs :
-    Timeless (ws_hub_model t vs).
+  #[global] Instance ws_hub_2_model_timeless t vs :
+    Timeless (ws_hub_2_model t vs).
   Proof.
     apply _.
   Qed.
-  #[global] Instance ws_hub_inv_persistent t ι :
-    Persistent (ws_hub_inv t ι).
+  #[global] Instance ws_hub_2_inv_persistent t ι :
+    Persistent (ws_hub_2_inv t ι).
   Proof.
     apply _.
   Qed.
 
-  #[local] Lemma ws_hub_model_alloc :
+  #[local] Lemma ws_hub_2_model_alloc :
     ⊢ |==>
       ∃ γ_model,
-      ws_hub_model₁' γ_model ∅ ∗
-      ws_hub_model₂' γ_model ∅.
+      ws_hub_2_model₁' γ_model ∅ ∗
+      ws_hub_2_model₂' γ_model ∅.
   Proof.
     apply twins_alloc'.
   Qed.
-  #[local] Lemma ws_hub_model_agree γ vs1 vs2 :
-    ws_hub_model₁ γ vs1 -∗
-    ws_hub_model₂ γ vs2 -∗
+  #[local] Lemma ws_hub_2_model_agree γ vs1 vs2 :
+    ws_hub_2_model₁ γ vs1 -∗
+    ws_hub_2_model₂ γ vs2 -∗
     ⌜vs1 = vs2⌝.
   Proof.
     apply: twins_agree_L.
   Qed.
-  #[local] Lemma ws_hub_model_update {γ vs1 vs2} vs :
-    ws_hub_model₁ γ vs1 -∗
-    ws_hub_model₂ γ vs2 ==∗
-      ws_hub_model₁ γ vs ∗
-      ws_hub_model₂ γ vs.
+  #[local] Lemma ws_hub_2_model_update {γ vs1 vs2} vs :
+    ws_hub_2_model₁ γ vs1 -∗
+    ws_hub_2_model₂ γ vs2 ==∗
+      ws_hub_2_model₁ γ vs ∗
+      ws_hub_2_model₂ γ vs.
   Proof.
     apply twins_update'.
   Qed.
 
-  Lemma ws_hub_owner_exclusive t i :
-    ws_hub_owner t i -∗
-    ws_hub_owner t i -∗
+  Lemma ws_hub_2_owner_exclusive t i :
+    ws_hub_2_owner t i -∗
+    ws_hub_2_owner t i -∗
     False.
   Proof.
     iIntros "(%l & %γ & %rounds & %n & -> & #Hmeta & _ & Howner1 & _) (%_l & %_γ & %_rounds & %_n & %Heq & #_Hmeta & _ & Howner2 & _)". injection Heq as <-.
@@ -367,16 +349,16 @@ Section ws_hub_G.
     iApply (ws_deques_owner_exclusive with "Howner1 Howner2").
   Qed.
 
-  Lemma ws_hub_create_spec ι sz :
+  Lemma ws_hub_2_create_spec ι sz :
     (0 ≤ sz)%Z →
     {{{ True }}}
-      ws_hub_create ws_deques #sz
+      ws_hub_2_create ws_deques #sz
     {{{ t,
       RET t;
-      ws_hub_inv t ι ∗
-      ws_hub_model t ∅ ∗
+      ws_hub_2_inv t ι ∗
+      ws_hub_2_model t ∅ ∗
       [∗ list] i ∈ seq 0 (Z.to_nat sz),
-        ws_hub_owner t i
+        ws_hub_2_owner t i
     }}}.
   Proof.
     set sz' := Z.to_nat sz.
@@ -402,15 +384,15 @@ Section ws_hub_G.
     iMod (pointsto_persist with "Hl_rounds") as "#Hl_rounds".
     iMod (pointsto_persist with "Hl_waiters") as "#Hl_waiters".
 
-    iMod ws_hub_model_alloc as "(%γ_model & Hmodel₁ & Hmodel₂)".
+    iMod ws_hub_2_model_alloc as "(%γ_model & Hmodel₁ & Hmodel₂)".
 
     pose γ := {|
-      ws_hub_meta_size := sz' ;
-      ws_hub_meta_deques := deques ;
-      ws_hub_meta_foreign := foreign ;
-      ws_hub_meta_rounds := v_rounds ;
-      ws_hub_meta_waiters := waiters ;
-      ws_hub_meta_model := γ_model ;
+      ws_hub_2_meta_size := sz' ;
+      ws_hub_2_meta_deques := deques ;
+      ws_hub_2_meta_foreign := foreign ;
+      ws_hub_2_meta_rounds := v_rounds ;
+      ws_hub_2_meta_waiters := waiters ;
+      ws_hub_2_meta_model := γ_model ;
     |}.
 
     iMod (meta_set _ _ γ with "Hmeta") as "#Hmeta"; first done.
@@ -430,11 +412,11 @@ Section ws_hub_G.
       rewrite Hrounds. iSteps.
   Qed.
 
-  #[local] Lemma ws_hub_num_worker_spec t ι :
+  #[local] Lemma ws_hub_2_num_worker_spec t ι :
     {{{
-      ws_hub_inv t ι
+      ws_hub_2_inv t ι
     }}}
-      ws_hub_num_worker t
+      ws_hub_2_num_worker t
     {{{ num_worker,
       RET #num_worker; True
     }}}.
@@ -442,11 +424,11 @@ Section ws_hub_G.
     iSteps.
   Qed.
 
-  #[local] Lemma ws_hub_num_thief_spec t ι :
+  #[local] Lemma ws_hub_2_num_thief_spec t ι :
     {{{
-      ws_hub_inv t ι
+      ws_hub_2_inv t ι
     }}}
-      ws_hub_num_thief t
+      ws_hub_2_num_thief t
     {{{ num_thief,
       RET #num_thief; True
     }}}.
@@ -454,11 +436,11 @@ Section ws_hub_G.
     iSteps.
   Qed.
 
-  #[local] Lemma ws_hub_incr_num_worker_spec t ι :
+  #[local] Lemma ws_hub_2_incr_num_worker_spec t ι :
     {{{
-      ws_hub_inv t ι
+      ws_hub_2_inv t ι
     }}}
-      ws_hub_incr_num_worker t
+      ws_hub_2_incr_num_worker t
     {{{ num_worker,
       RET #num_worker; True
     }}}.
@@ -466,11 +448,11 @@ Section ws_hub_G.
     iSteps.
   Qed.
 
-  #[local] Lemma ws_hub_decr_num_worker_spec t ι :
+  #[local] Lemma ws_hub_2_decr_num_worker_spec t ι :
     {{{
-      ws_hub_inv t ι
+      ws_hub_2_inv t ι
     }}}
-      ws_hub_decr_num_worker t
+      ws_hub_2_decr_num_worker t
     {{{ num_worker,
       RET #num_worker; True
     }}}.
@@ -478,11 +460,11 @@ Section ws_hub_G.
     iSteps.
   Qed.
 
-  #[local] Lemma ws_hub_incr_num_thief_spec t ι :
+  #[local] Lemma ws_hub_2_incr_num_thief_spec t ι :
     {{{
-      ws_hub_inv t ι
+      ws_hub_2_inv t ι
     }}}
-      ws_hub_incr_num_thief t
+      ws_hub_2_incr_num_thief t
     {{{ num_thief,
       RET #num_thief; True
     }}}.
@@ -490,11 +472,11 @@ Section ws_hub_G.
     iSteps.
   Qed.
 
-  #[local] Lemma ws_hub_decr_num_thief_spec t ι :
+  #[local] Lemma ws_hub_2_decr_num_thief_spec t ι :
     {{{
-      ws_hub_inv t ι
+      ws_hub_2_inv t ι
     }}}
-      ws_hub_decr_num_thief t
+      ws_hub_2_decr_num_thief t
     {{{ num_thief,
       RET #num_thief; True
     }}}.
@@ -502,11 +484,11 @@ Section ws_hub_G.
     iSteps.
   Qed.
 
-  #[local] Lemma ws_hub_notify_spec t ι :
+  #[local] Lemma ws_hub_2_notify_spec t ι :
     {{{
-      ws_hub_inv t ι
+      ws_hub_2_inv t ι
     }}}
-      ws_hub_notify t
+      ws_hub_2_notify t
     {{{
       RET (); True
     }}}.
@@ -517,19 +499,19 @@ Section ws_hub_G.
     wp_apply (waiters_notify_spec with "Hwaiters_inv HΦ").
   Qed.
 
-  Lemma ws_hub_push_spec t ι i v :
+  Lemma ws_hub_2_push_spec t ι i v :
     (0 ≤ i)%Z →
     <<<
-      ws_hub_inv t ι ∗
-      ws_hub_owner t (Z.to_nat i)
+      ws_hub_2_inv t ι ∗
+      ws_hub_2_owner t (Z.to_nat i)
     | ∀∀ vs,
-      ws_hub_model t vs
+      ws_hub_2_model t vs
     >>>
-      ws_hub_push ws_deques t #i v @ ↑ι
+      ws_hub_2_push ws_deques t #i v @ ↑ι
     <<<
-      ws_hub_model t ({[+v+]} ⊎ vs)
+      ws_hub_2_model t ({[+v+]} ⊎ vs)
     | RET ();
-      ws_hub_owner t (Z.to_nat i)
+      ws_hub_2_owner t (Z.to_nat i)
     >>>.
   Proof.
     iIntros "%Hi !> %Φ ((%l & %γ & -> & #Hmeta & #Hl_deques & #Hl_foreign & #Hl_waiters & #Hdeques_inv & #Hforeign_inv & #Hwaiters_inv & #Hinv) & (%_l & %_γ & %round & %n & %Heq & _Hmeta & #Hl_rounds & Hdeques_owner & #Hv_rounds & Hround)) HΦ". injection Heq as <-.
@@ -541,14 +523,14 @@ Section ws_hub_G.
     iInv "Hinv" as "(%vs & %vss & %vs_foreign & %num_worker & %num_thief & >%Hvs & Hl_num_worker & Hl_num_thief & >Hdeques_model & Hforeign_model & >Hmodel₂)".
     iApply (aacc_aupd_commit with "HΦ"); first solve_ndisj. iIntros "%_vs (%_l & %_γ & %Heq & _Hmeta & Hmodel₁)". injection Heq as <-.
     iDestruct (meta_agree with "Hmeta _Hmeta") as %<-. iClear "_Hmeta".
-    iDestruct (ws_hub_model_agree with "Hmodel₁ Hmodel₂") as %->.
+    iDestruct (ws_hub_2_model_agree with "Hmodel₁ Hmodel₂") as %->.
     iAaccIntro with "Hdeques_model".
     { iIntros "Hdeques_model !>".
       iSplitL "Hmodel₁"; first iSteps. iIntros "$ !>".
       iSteps.
     }
     iIntros "%vs' (%Hlookup & Hdeques_model)".
-    iMod (ws_hub_model_update ({[+v+]} ⊎ vs) with "Hmodel₁ Hmodel₂") as "(Hmodel₁ & Hmodel₂)".
+    iMod (ws_hub_2_model_update ({[+v+]} ⊎ vs) with "Hmodel₁ Hmodel₂") as "(Hmodel₁ & Hmodel₂)".
     iSplitL "Hmodel₁"; first iSteps. iIntros "!> HΦ !>".
     iSplitR "HΦ".
     { repeat iExists _. iFrame. iPureIntro.
@@ -560,15 +542,15 @@ Section ws_hub_G.
     iSteps.
   Qed.
 
-  Lemma ws_hub_push_foreign_spec t ι v :
+  Lemma ws_hub_2_push_foreign_spec t ι v :
     <<<
-      ws_hub_inv t ι
+      ws_hub_2_inv t ι
     | ∀∀ vs,
-      ws_hub_model t vs
+      ws_hub_2_model t vs
     >>>
-      ws_hub_push_foreign ws_deques t v @ ↑ι
+      ws_hub_2_push_foreign ws_deques t v @ ↑ι
     <<<
-      ws_hub_model t ({[+v+]} ⊎ vs)
+      ws_hub_2_model t ({[+v+]} ⊎ vs)
     | RET (); True
     >>>.
   Proof.
@@ -580,14 +562,14 @@ Section ws_hub_G.
     iInv "Hinv" as "(%vs & %vss & %vs_foreign & %num_worker & %num_thief & >%Hvs & Hl_num_worker & Hl_num_thief & Hdeques_model & >Hforeign_model & >Hmodel₂)".
     iApply (aacc_aupd_commit with "HΦ"); first solve_ndisj. iIntros "%_vs (%_l & %_γ & %Heq & _Hmeta & Hmodel₁)". injection Heq as <-.
     iDestruct (meta_agree with "Hmeta _Hmeta") as %<-. iClear "_Hmeta".
-    iDestruct (ws_hub_model_agree with "Hmodel₁ Hmodel₂") as %->.
+    iDestruct (ws_hub_2_model_agree with "Hmodel₁ Hmodel₂") as %->.
     iAaccIntro with "Hforeign_model".
     { iIntros "Hforeign_model !>".
       iSplitL "Hmodel₁"; first iSteps. iIntros "$ !>".
       iSteps.
     }
     iIntros "Hforeign_model".
-    iMod (ws_hub_model_update ({[+v+]} ⊎ vs) with "Hmodel₁ Hmodel₂") as "(Hmodel₁ & Hmodel₂)".
+    iMod (ws_hub_2_model_update ({[+v+]} ⊎ vs) with "Hmodel₁ Hmodel₂") as "(Hmodel₁ & Hmodel₂)".
     iSplitL "Hmodel₁"; first iSteps. iIntros "!> HΦ !>".
     iSplitR "HΦ".
     { repeat iExists _. iFrame. iPureIntro.
@@ -597,27 +579,27 @@ Section ws_hub_G.
     iSteps.
   Qed.
 
-  Lemma ws_hub_pop_spec t ι i :
+  Lemma ws_hub_2_pop_spec t ι i :
     (0 ≤ i)%Z →
     <<<
-      ws_hub_inv t ι ∗
-      ws_hub_owner t (Z.to_nat i)
+      ws_hub_2_inv t ι ∗
+      ws_hub_2_owner t (Z.to_nat i)
     | ∀∀ vs,
-      ws_hub_model t vs
+      ws_hub_2_model t vs
     >>>
-      ws_hub_pop ws_deques t #i @ ↑ι
+      ws_hub_2_pop ws_deques t #i @ ↑ι
     <<<
       ∃∃ o,
       match o with
       | None =>
-          ws_hub_model t vs
+          ws_hub_2_model t vs
       | Some v =>
           ∃ vs',
           ⌜vs = {[+v+]} ⊎ vs'⌝ ∗
-          ws_hub_model t vs'
+          ws_hub_2_model t vs'
       end
     | RET o;
-      ws_hub_owner t (Z.to_nat i)
+      ws_hub_2_owner t (Z.to_nat i)
     >>>.
   Proof.
     iIntros "%Hi !> %Φ ((%l & %γ & -> & #Hmeta & #Hl_deques & #Hl_foreign & #Hl_waiters & #Hdeques_inv & #Hforeign_inv & #Hwaiters_inv & #Hinv) & (%_l & %_γ & %round & %n & %Heq & _Hmeta & #Hl_rounds & Hdeques_owner & #Hv_rounds & Hround)) HΦ". injection Heq as <-.
@@ -629,7 +611,7 @@ Section ws_hub_G.
     iInv "Hinv" as "(%vs & %vss & %vs_foreign & %num_worker & %num_thief & >%Hvs & Hl_num_worker & Hl_num_thief & >Hdeques_model & Hforeign_model & >Hmodel₂)".
     iApply (aacc_aupd_commit with "HΦ"); first solve_ndisj. iIntros "%_vs (%_l & %_γ & %Heq & _Hmeta & Hmodel₁)". injection Heq as <-.
     iDestruct (meta_agree with "Hmeta _Hmeta") as %<-. iClear "_Hmeta".
-    iDestruct (ws_hub_model_agree with "Hmodel₁ Hmodel₂") as %->.
+    iDestruct (ws_hub_2_model_agree with "Hmodel₁ Hmodel₂") as %->.
     iAaccIntro with "Hdeques_model".
     { iIntros "Hdeques_model !>".
       iSplitL "Hmodel₁"; first iSteps.
@@ -639,7 +621,7 @@ Section ws_hub_G.
 
     - iDestruct "Hdeques_model" as "(%ws & %Hlookup & Hdeques_model)".
       set vs' := vs ∖ {[+v+]}.
-      iMod (ws_hub_model_update vs' with "Hmodel₁ Hmodel₂") as "(Hmodel₁ & Hmodel₂)".
+      iMod (ws_hub_2_model_update vs' with "Hmodel₁ Hmodel₂") as "(Hmodel₁ & Hmodel₂)".
       iExists (Some v).
       iSplitL "Hmodel₁".
       { iExists vs'. iSteps. iPureIntro.
@@ -666,22 +648,22 @@ Section ws_hub_G.
       iSplitR "HΦ"; iSteps.
   Qed.
 
-  #[local] Lemma ws_hub_pop_foreign_spec t ι :
+  #[local] Lemma ws_hub_2_pop_foreign_spec t ι :
     <<<
-      ws_hub_inv t ι
+      ws_hub_2_inv t ι
     | ∀∀ vs,
-      ws_hub_model t vs
+      ws_hub_2_model t vs
     >>>
-      ws_hub_pop_foreign t @ ↑ι
+      ws_hub_2_pop_foreign t @ ↑ι
     <<<
       ∃∃ o,
       match o with
       | None =>
-          ws_hub_model t vs
+          ws_hub_2_model t vs
       | Some v =>
           ∃ vs',
           ⌜vs = {[+v+]} ⊎ vs'⌝ ∗
-          ws_hub_model t vs'
+          ws_hub_2_model t vs'
       end
     | RET o; True
     >>>.
@@ -694,7 +676,7 @@ Section ws_hub_G.
     iInv "Hinv" as "(%vs & %vss & %vs_foreign & %num_worker & %num_thief & >%Hvs & Hl_num_worker & Hl_num_thief & Hdeques_model & >Hforeign_model & >Hmodel₂)".
     iApply (aacc_aupd_commit with "HΦ"); first solve_ndisj. iIntros "%_vs (%_l & %_γ & %Heq & _Hmeta & Hmodel₁)". injection Heq as <-.
     iDestruct (meta_agree with "Hmeta _Hmeta") as %<-. iClear "_Hmeta".
-    iDestruct (ws_hub_model_agree with "Hmodel₁ Hmodel₂") as %->.
+    iDestruct (ws_hub_2_model_agree with "Hmodel₁ Hmodel₂") as %->.
     iAaccIntro with "Hforeign_model".
     { iIntros "Hforeign_model !>".
       iSplitL "Hmodel₁"; first iSteps.
@@ -709,7 +691,7 @@ Section ws_hub_G.
       iSplitR "HΦ"; iSteps.
 
     - set vs' := vs ∖ {[+v+]}.
-      iMod (ws_hub_model_update vs' with "Hmodel₁ Hmodel₂") as "(Hmodel₁ & Hmodel₂)".
+      iMod (ws_hub_2_model_update vs' with "Hmodel₁ Hmodel₂") as "(Hmodel₁ & Hmodel₂)".
       iExists (Some v).
       iSplitL "Hmodel₁".
       { iExists vs'. iSteps. iPureIntro.
@@ -726,27 +708,27 @@ Section ws_hub_G.
       iSteps.
   Qed.
 
-  #[local] Lemma ws_hub_try_steal_once_spec t ι i :
+  #[local] Lemma ws_hub_2_try_steal_once_spec t ι i :
     (0 ≤ i)%Z →
     <<<
-      ws_hub_inv t ι ∗
-      ws_hub_owner t (Z.to_nat i)
+      ws_hub_2_inv t ι ∗
+      ws_hub_2_owner t (Z.to_nat i)
     | ∀∀ vs,
-      ws_hub_model t vs
+      ws_hub_2_model t vs
     >>>
-      ws_hub_try_steal_once ws_deques t #i @ ↑ι
+      ws_hub_2_try_steal_once ws_deques t #i @ ↑ι
     <<<
       ∃∃ o,
       match o with
       | None =>
-          ws_hub_model t vs
+          ws_hub_2_model t vs
       | Some v =>
           ∃ vs',
           ⌜vs = {[+v+]} ⊎ vs'⌝ ∗
-          ws_hub_model t vs'
+          ws_hub_2_model t vs'
       end
     | RET o;
-      ws_hub_owner t (Z.to_nat i)
+      ws_hub_2_owner t (Z.to_nat i)
     >>>.
   Proof.
     iIntros "%Hi !> %Φ ((%l & %γ & -> & #Hmeta & #Hl_deques & #Hl_foreign & #Hl_waiters & #Hdeques_inv & #Hforeign_inv & #Hwaiters_inv & #Hinv) & (%_l & %_γ & %round & %n & %Heq & _Hmeta & #Hl_rounds & Hdeques_owner & #Hv_rounds & Hround)) HΦ". injection Heq as <-.
@@ -762,7 +744,7 @@ Section ws_hub_G.
     iInv "Hinv" as "(%vs & %vss & %vs_foreign & %num_worker & %num_thief & >%Hvs & Hl_num_worker & Hl_num_thief & >Hdeques_model & Hforeign_model & >Hmodel₂)".
     iApply (aacc_aupd_commit with "HΦ"); first solve_ndisj. iIntros "%_vs (%_l & %_γ & %Heq & _Hmeta & Hmodel₁)". injection Heq as <-.
     iDestruct (meta_agree with "Hmeta _Hmeta") as %<-. iClear "_Hmeta".
-    iDestruct (ws_hub_model_agree with "Hmodel₁ Hmodel₂") as %->.
+    iDestruct (ws_hub_2_model_agree with "Hmodel₁ Hmodel₂") as %->.
     iAaccIntro with "Hdeques_model".
     { iIntros "Hdeques_model !>".
       iSplitL "Hmodel₁"; first iSteps.
@@ -772,7 +754,7 @@ Section ws_hub_G.
 
     - iDestruct "Hdeques_model" as "(%j & %ws & %Hj & %Hlookup & Hdeques_model)".
       set vs' := vs ∖ {[+v+]}.
-      iMod (ws_hub_model_update vs' with "Hmodel₁ Hmodel₂") as "(Hmodel₁ & Hmodel₂)".
+      iMod (ws_hub_2_model_update vs' with "Hmodel₁ Hmodel₂") as "(Hmodel₁ & Hmodel₂)".
       iExists (Some v).
       iSplitL "Hmodel₁".
       { iExists vs'. iSteps. iPureIntro.
@@ -797,28 +779,28 @@ Section ws_hub_G.
       iSplitR "HΦ"; iSteps.
   Qed.
 
-  #[local] Lemma ws_hub_try_steal_aux_spec yield t ι i max_round :
+  #[local] Lemma ws_hub_2_try_steal_aux_spec yield t ι i max_round :
     (0 ≤ i)%Z →
     (0 ≤ max_round)%Z →
     <<<
-      ws_hub_inv t ι ∗
-      ws_hub_owner t (Z.to_nat i)
+      ws_hub_2_inv t ι ∗
+      ws_hub_2_owner t (Z.to_nat i)
     | ∀∀ vs,
-      ws_hub_model t vs
+      ws_hub_2_model t vs
     >>>
-      ws_hub_try_steal_aux ws_deques yield t #i #max_round @ ↑ι
+      ws_hub_2_try_steal_aux ws_deques yield t #i #max_round @ ↑ι
     <<<
       ∃∃ o,
       match o with
       | None =>
-          ws_hub_model t vs
+          ws_hub_2_model t vs
       | Some v =>
           ∃ vs',
           ⌜vs = {[+v+]} ⊎ vs'⌝ ∗
-          ws_hub_model t vs'
+          ws_hub_2_model t vs'
       end
     | RET o;
-      ws_hub_owner t (Z.to_nat i)
+      ws_hub_2_owner t (Z.to_nat i)
     >>>.
   Proof.
     intros Hi.
@@ -834,7 +816,7 @@ Section ws_hub_G.
       iApply ("HΦ" $! None with "Hmodel").
       iSteps.
 
-    - awp_apply ws_hub_pop_foreign_spec without "Hdeques_owner Hround"; first iSteps.
+    - awp_apply ws_hub_2_pop_foreign_spec without "Hdeques_owner Hround"; first iSteps.
       iApply (aacc_aupd with "HΦ"); first done. iIntros "%vs Hmodel".
       iAaccIntro with "Hmodel"; first iSteps. iIntros ([v |]) "Hmodel !>".
 
@@ -844,7 +826,7 @@ Section ws_hub_G.
       + iLeft. iFrame.
         iIntros "HΦ !> _ (Hdeques_owner & Hround)". clear- Hi Hmax_round Hcase.
 
-        awp_smart_apply (ws_hub_try_steal_once_spec with "[Hdeques_owner Hround]"); [done | iSteps |].
+        awp_smart_apply (ws_hub_2_try_steal_once_spec with "[Hdeques_owner Hround]"); [done | iSteps |].
         iApply (aacc_aupd with "HΦ"); first done. iIntros "%vs Hmodel".
         iAaccIntro with "Hmodel"; first iSteps. iIntros ([v |]) "Hmodel !>".
 
@@ -863,36 +845,36 @@ Section ws_hub_G.
           { destruct yield; iSteps. }
           wp_smart_apply ("HLöb" with "[] [$Howner] HΦ"); iSteps.
   Qed.
-  Lemma ws_hub_try_steal_spec t ι i max_round_noyield max_round_yield :
+  Lemma ws_hub_2_try_steal_spec t ι i max_round_noyield max_round_yield :
     (0 ≤ i)%Z →
     (0 ≤ max_round_noyield)%Z →
     (0 ≤ max_round_yield)%Z →
     <<<
-      ws_hub_inv t ι ∗
-      ws_hub_owner t (Z.to_nat i)
+      ws_hub_2_inv t ι ∗
+      ws_hub_2_owner t (Z.to_nat i)
     | ∀∀ vs,
-      ws_hub_model t vs
+      ws_hub_2_model t vs
     >>>
-      ws_hub_try_steal ws_deques t #i (#max_round_noyield, #max_round_yield)%V @ ↑ι
+      ws_hub_2_try_steal ws_deques t #i (#max_round_noyield, #max_round_yield)%V @ ↑ι
     <<<
       ∃∃ o,
       match o with
       | None =>
-          ws_hub_model t vs
+          ws_hub_2_model t vs
       | Some v =>
           ∃ vs',
           ⌜vs = {[+v+]} ⊎ vs'⌝ ∗
-          ws_hub_model t vs'
+          ws_hub_2_model t vs'
       end
     | RET o;
-      ws_hub_owner t (Z.to_nat i)
+      ws_hub_2_owner t (Z.to_nat i)
     >>>.
   Proof.
     iIntros "%Hi %Hmax_round_noyield %Hmax_round_yield !> %Φ (#Hinv & Howner) HΦ".
 
     wp_rec.
 
-    awp_smart_apply (ws_hub_try_steal_aux_spec with "[$Hinv $Howner]"); [done.. |].
+    awp_smart_apply (ws_hub_2_try_steal_aux_spec with "[$Hinv $Howner]"); [done.. |].
     iApply (aacc_aupd with "HΦ"); first done. iIntros "%vs Hmodel".
     iAaccIntro with "Hmodel"; first iSteps. iIntros ([v |]) "Hmodel !>".
 
@@ -905,82 +887,37 @@ Section ws_hub_G.
     - iLeft. iFrame.
       iIntros "HΦ !> Howner". clear- Hi Hmax_round_yield.
 
-      wp_smart_apply (ws_hub_try_steal_aux_spec with "[$Hinv $Howner] HΦ"); done.
+      wp_smart_apply (ws_hub_2_try_steal_aux_spec with "[$Hinv $Howner] HΦ"); done.
   Qed.
 
-  Lemma ws_hub_pop_try_steal_spec t ι i max_round_noyield max_round_yield :
-    (0 ≤ i)%Z →
-    (0 ≤ max_round_noyield)%Z →
-    (0 ≤ max_round_yield)%Z →
-    <<<
-      ws_hub_inv t ι ∗
-      ws_hub_owner t (Z.to_nat i)
-    | ∀∀ vs,
-      ws_hub_model t vs
-    >>>
-      ws_hub_pop_try_steal ws_deques t #i (#max_round_noyield, #max_round_yield)%V @ ↑ι
-    <<<
-      ∃∃ o,
-      match o with
-      | None =>
-          ws_hub_model t vs
-      | Some v =>
-          ∃ vs',
-          ⌜vs = {[+v+]} ⊎ vs'⌝ ∗
-          ws_hub_model t vs'
-      end
-    | RET o;
-      ws_hub_owner t (Z.to_nat i)
-    >>>.
-  Proof.
-    iIntros "%Hi %Hmax_round_noyield %Hmax_round_yield !> %Φ (#Hinv & Howner) HΦ".
-
-    wp_rec.
-
-    awp_smart_apply (ws_hub_pop_spec with "[$Hinv $Howner]"); [done.. |].
-    iApply (aacc_aupd with "HΦ"); first done. iIntros "%vs Hmodel".
-    iAaccIntro with "Hmodel"; first iSteps. iIntros ([v |]) "Hmodel !>".
-
-    - iRight. iExists (Some v). iFrame.
-      iIntros "HΦ !> Howner". clear.
-
-      iSpecialize ("HΦ" with "Howner").
-      iSteps.
-
-    - iLeft. iFrame.
-      iIntros "HΦ !> Howner". clear- Hi Hmax_round_noyield Hmax_round_yield.
-
-      wp_smart_apply (ws_hub_try_steal_spec with "[$Hinv $Howner] HΦ"); done.
-  Qed.
-
-  #[local] Lemma ws_hub_steal_init_spec t ι :
+  #[local] Lemma ws_hub_2_steal_init_spec t ι :
     {{{
-      ws_hub_inv t ι
+      ws_hub_2_inv t ι
     }}}
-      ws_hub_steal_init t
+      ws_hub_2_steal_init t
     {{{
       RET (); True
     }}}.
   Proof.
     iSteps.
   Qed.
-  #[local] Lemma ws_hub_steal_2_spec t ι i max_round_noyield max_round_yield :
+  #[local] Lemma ws_hub_2_steal_2_spec t ι i max_round_noyield max_round_yield :
     (0 ≤ i)%Z →
     (0 ≤ max_round_noyield)%Z →
     (0 ≤ max_round_yield)%Z →
     <<<
-      ws_hub_inv t ι ∗
-      ws_hub_owner t (Z.to_nat i)
+      ws_hub_2_inv t ι ∗
+      ws_hub_2_owner t (Z.to_nat i)
     | ∀∀ vs,
-      ws_hub_model t vs
+      ws_hub_2_model t vs
     >>>
-      ws_hub_steal_2 ws_deques t #i (#max_round_noyield, #max_round_yield)%V @ ↑ι
+      ws_hub_2_steal_2 ws_deques t #i (#max_round_noyield, #max_round_yield)%V @ ↑ι
     <<<
       ∃∃ v vs',
       ⌜vs = {[+v+]} ⊎ vs'⌝ ∗
-      ws_hub_model t vs'
+      ws_hub_2_model t vs'
     | RET v;
-      ws_hub_owner t (Z.to_nat i)
+      ws_hub_2_owner t (Z.to_nat i)
     >>>.
   Proof.
     iIntros "%Hi %Hmax_round_noyield %Hmax_round_yield !> %Φ (#Hinv & Howner) HΦ".
@@ -989,7 +926,7 @@ Section ws_hub_G.
 
     wp_rec.
 
-    awp_smart_apply (ws_hub_try_steal_spec with "[$Hinv $Howner]"); [done.. |].
+    awp_smart_apply (ws_hub_2_try_steal_spec with "[$Hinv $Howner]"); [done.. |].
     iApply (aacc_aupd with "HΦ"); first done. iIntros "%vs Hmodel".
     iAaccIntro with "Hmodel"; first iSteps. iIntros ([v |]) "Hmodel !>".
 
@@ -1017,20 +954,20 @@ Section ws_hub_G.
         wp_apply (wp_wand _ _ (λ res, ⌜res = ()%V⌝)%I with "[Hwaiter]") as (res) "->".
         { wp_bind (_ and _)%E.
           wp_apply (wp_wand _ _ (λ res, ∃ b, ⌜res = #b⌝)%I) as (res) "(%b & ->)".
-          { wp_apply ws_hub_decr_num_thief_spec as (num_thief) "_"; first iSteps.
+          { wp_apply ws_hub_2_decr_num_thief_spec as (num_thief) "_"; first iSteps.
             wp_pures. case_bool_decide as Hcase; wp_pures; last iSteps.
-            wp_apply ws_hub_num_worker_spec as (num_worker) "_"; first iSteps.
+            wp_apply ws_hub_2_num_worker_spec as (num_worker) "_"; first iSteps.
             iSteps.
           }
           destruct b.
           - wp_smart_apply (waiters_cancel_wait_spec with "[$Hwaiters_inv $Hwaiter]") as "_ //".
           - wp_smart_apply (waiters_commit_wait_spec with "[$Hwaiters_inv $Hwaiter]") as "_ //".
         }
-        wp_smart_apply ws_hub_steal_init_spec as "_"; first iSteps.
+        wp_smart_apply ws_hub_2_steal_init_spec as "_"; first iSteps.
         wp_smart_apply ("HLöb" with "Howner HΦ").
 
       + wp_smart_apply (waiters_cancel_wait_spec with "[$Hwaiters_inv $Hwaiter]") as "_".
-        awp_smart_apply ws_hub_pop_foreign_spec; first iSteps.
+        awp_smart_apply ws_hub_2_pop_foreign_spec; first iSteps.
         iApply (aacc_aupd with "HΦ"); first done. iIntros "%vs Hmodel".
         iAaccIntro with "Hmodel"; first iIntros "$ !> $ //". iIntros ([v |]) "Hmodel !>".
 
@@ -1046,66 +983,66 @@ Section ws_hub_G.
 
           wp_smart_apply ("HLöb" with "Howner HΦ").
   Qed.
-  #[local] Lemma ws_hub_steal_1_spec t ι i max_round_noyield max_round_yield :
+  #[local] Lemma ws_hub_2_steal_1_spec t ι i max_round_noyield max_round_yield :
     (0 ≤ i)%Z →
     (0 ≤ max_round_noyield)%Z →
     (0 ≤ max_round_yield)%Z →
     <<<
-      ws_hub_inv t ι ∗
-      ws_hub_owner t (Z.to_nat i)
+      ws_hub_2_inv t ι ∗
+      ws_hub_2_owner t (Z.to_nat i)
     | ∀∀ vs,
-      ws_hub_model t vs
+      ws_hub_2_model t vs
     >>>
-      ws_hub_steal_1 ws_deques t #i (#max_round_noyield, #max_round_yield)%V @ ↑ι
+      ws_hub_2_steal_1 ws_deques t #i (#max_round_noyield, #max_round_yield)%V @ ↑ι
     <<<
       ∃∃ v vs',
       ⌜vs = {[+v+]} ⊎ vs'⌝ ∗
-      ws_hub_model t vs'
+      ws_hub_2_model t vs'
     | RET v;
-      ws_hub_owner t (Z.to_nat i)
+      ws_hub_2_owner t (Z.to_nat i)
     >>>.
   Proof.
     iIntros "%Hi %Hmax_round_noyield %Hmax_round_yield !> %Φ (#Hinv & Howner)HΦ".
 
     wp_rec.
-    wp_smart_apply (ws_hub_steal_init_spec with "Hinv") as "_".
+    wp_smart_apply (ws_hub_2_steal_init_spec with "Hinv") as "_".
 
-    awp_smart_apply (ws_hub_steal_2_spec with "[$Hinv $Howner]"); [done.. |].
+    awp_smart_apply (ws_hub_2_steal_2_spec with "[$Hinv $Howner]"); [done.. |].
     iApply (aacc_aupd_commit with "HΦ"); first done. iIntros "%vs Hmodel".
     iAaccIntro with "Hmodel"; first iSteps. iIntros "%v %vs' (-> & Hmodel) !>".
     iExists v, vs'. iFrame. iStep. iIntros "HΦ !> Howner".
 
-    wp_smart_apply (ws_hub_decr_num_thief_spec with "Hinv") as (num_thief) "_".
+    wp_smart_apply (ws_hub_2_decr_num_thief_spec with "Hinv") as (num_thief) "_".
     wp_pures. case_bool_decide as Hcase; wp_pures; last by iStep.
-    wp_apply (ws_hub_notify_spec with "Hinv") as "_".
+    wp_apply (ws_hub_2_notify_spec with "Hinv") as "_".
     wp_pures.
     by iStep.
   Qed.
-  Lemma ws_hub_steal_spec t ι i max_round_noyield max_round_yield :
+  Lemma ws_hub_2_steal_spec t ι i max_round_noyield max_round_yield :
     (0 ≤ i)%Z →
     (0 ≤ max_round_noyield)%Z →
     (0 ≤ max_round_yield)%Z →
     <<<
-      ws_hub_inv t ι ∗
-      ws_hub_owner t (Z.to_nat i)
+      ws_hub_2_inv t ι ∗
+      ws_hub_2_owner t (Z.to_nat i)
     | ∀∀ vs,
-      ws_hub_model t vs
+      ws_hub_2_model t vs
     >>>
-      ws_hub_steal ws_deques t #i (#max_round_noyield, #max_round_yield)%V @ ↑ι
+      ws_hub_2_steal ws_deques t #i (#max_round_noyield, #max_round_yield)%V @ ↑ι
     <<<
       ∃∃ v vs',
       ⌜vs = {[+v+]} ⊎ vs'⌝ ∗
-      ws_hub_model t vs'
+      ws_hub_2_model t vs'
     | RET v;
-      ws_hub_owner t (Z.to_nat i)
+      ws_hub_2_owner t (Z.to_nat i)
     >>>.
   Proof.
     iIntros "%Hi %Hmax_round_noyield %Hmax_round_yield !> %Φ (#Hinv & Howner)HΦ".
 
     wp_rec.
-    wp_smart_apply (ws_hub_decr_num_worker_spec with "Hinv") as (num_worker_1) "_".
+    wp_smart_apply (ws_hub_2_decr_num_worker_spec with "Hinv") as (num_worker_1) "_".
 
-    awp_smart_apply (ws_hub_steal_1_spec with "[$Hinv $Howner]"); [done.. |].
+    awp_smart_apply (ws_hub_2_steal_1_spec with "[$Hinv $Howner]"); [done.. |].
     iApply (aacc_aupd_commit with "HΦ"); first done. iIntros "%vs Hmodel".
     iAaccIntro with "Hmodel"; first iSteps. iIntros "%v %vs' (-> & Hmodel) !>".
     iExists v, vs'. iFrame. iStep. iIntros "HΦ !> Howner".
@@ -1115,69 +1052,37 @@ Section ws_hub_G.
     wp_apply (wp_wand _ _ (λ res, ⌜res = ()%V⌝)%I) as (res) "->".
     { wp_bind (_ and _)%E.
       wp_apply (wp_wand _ _ (λ res, ∃ b, ⌜res = #b⌝)%I) as (res) "(%b & ->)".
-      { wp_apply (ws_hub_incr_num_worker_spec with "Hinv") as (num_worker_2) "_".
+      { wp_apply (ws_hub_2_incr_num_worker_spec with "Hinv") as (num_worker_2) "_".
         wp_pures. case_bool_decide as Hcase; wp_pures; last iSteps.
-        wp_apply (ws_hub_num_thief_spec with "Hinv") as (num_thief) "_".
+        wp_apply (ws_hub_2_num_thief_spec with "Hinv") as (num_thief) "_".
         iSteps.
       }
       destruct b; last iSteps.
-      wp_smart_apply (ws_hub_notify_spec with "Hinv") as "_".
+      wp_smart_apply (ws_hub_2_notify_spec with "Hinv") as "_".
       iSteps.
     }
     wp_pures.
     by iStep.
   Qed.
 
-  Lemma ws_hub_pop_steal_spec t ι i max_round_noyield max_round_yield :
-    (0 ≤ i)%Z →
-    (0 ≤ max_round_noyield)%Z →
-    (0 ≤ max_round_yield)%Z →
-    <<<
-      ws_hub_inv t ι ∗
-      ws_hub_owner t (Z.to_nat i)
-    | ∀∀ vs,
-      ws_hub_model t vs
-    >>>
-      ws_hub_pop_steal ws_deques t #i (#max_round_noyield, #max_round_yield)%V @ ↑ι
-    <<<
-      ∃∃ v vs',
-      ⌜vs = {[+v+]} ⊎ vs'⌝ ∗
-      ws_hub_model t vs'
-    | RET v;
-      ws_hub_owner t (Z.to_nat i)
-    >>>.
-  Proof.
-    iIntros "%Hi %Hmax_round_noyield %Hmax_round_yield !> %Φ (#Hinv & Howner) HΦ".
+  Definition ws_hub_2 :=
+    Build_ws_hub
+      ws_hub_2_owner_exclusive
+      ws_hub_2_create_spec
+      ws_hub_2_push_spec
+      ws_hub_2_push_foreign_spec
+      ws_hub_2_pop_spec
+      ws_hub_2_try_steal_spec
+      ws_hub_2_steal_spec.
+End ws_hub_2_G.
 
-    wp_rec.
+#[global] Opaque ws_hub_2_create.
+#[global] Opaque ws_hub_2_push.
+#[global] Opaque ws_hub_2_push_foreign.
+#[global] Opaque ws_hub_2_pop.
+#[global] Opaque ws_hub_2_try_steal.
+#[global] Opaque ws_hub_2_steal.
 
-    awp_smart_apply (ws_hub_pop_spec with "[$Hinv $Howner]"); [done.. |].
-    iApply (aacc_aupd with "HΦ"); first done. iIntros "%vs Hmodel".
-    iAaccIntro with "Hmodel"; first iSteps. iIntros ([v |]) "Hmodel !>".
-
-    - iDestruct "Hmodel" as "(%vs' & -> & Hmodel)".
-      iRight. iExists v, vs'. iFrame. iStep.
-      iIntros "HΦ !> Howner". clear.
-
-      iSpecialize ("HΦ" with "Howner").
-      iSteps.
-
-    - iLeft. iFrame.
-      iIntros "HΦ !> Howner". clear- Hi Hmax_round_noyield Hmax_round_yield.
-
-      wp_smart_apply (ws_hub_steal_spec with "[$Hinv $Howner] HΦ"); done.
-  Qed.
-End ws_hub_G.
-
-#[global] Opaque ws_hub_create.
-#[global] Opaque ws_hub_push.
-#[global] Opaque ws_hub_push_foreign.
-#[global] Opaque ws_hub_pop.
-#[global] Opaque ws_hub_try_steal.
-#[global] Opaque ws_hub_pop_try_steal.
-#[global] Opaque ws_hub_steal.
-#[global] Opaque ws_hub_pop_steal.
-
-#[global] Opaque ws_hub_inv.
-#[global] Opaque ws_hub_model.
-#[global] Opaque ws_hub_owner.
+#[global] Opaque ws_hub_2_inv.
+#[global] Opaque ws_hub_2_model.
+#[global] Opaque ws_hub_2_owner.
