theories/parabstr/ws_hub.v
@@ -1,0 +1,261 @@
+From zebre Require Import
+  prelude.
+From zebre.language Require Import
+  notations
+  diaframe.
+From zebre.std Require Import
+  opt.
+From zebre.parabstr Require Export
+  base.
+From zebre Require Import
+  options.
+
+Implicit Types v t : val.
+
+Record ws_hub `{zebre_G : !ZebreG Σ} := {
+  ws_hub_create : val ;
+  ws_hub_push : val ;
+  ws_hub_push_foreign : val ;
+  ws_hub_pop : val ;
+  ws_hub_try_steal : val ;
+  ws_hub_steal : val ;
+
+  ws_hub_inv : val → namespace → iProp Σ ;
+  ws_hub_model : val → gmultiset val → iProp Σ ;
+  ws_hub_owner : val → nat → iProp Σ ;
+
+  #[global] ws_hub_model_timeless t vs ::
+    Timeless (ws_hub_model t vs) ;
+  #[global] ws_hub_inv_persistent t ι ::
+    Persistent (ws_hub_inv t ι) ;
+
+  ws_hub_owner_exclusive t i :
+    ws_hub_owner t i -∗
+    ws_hub_owner t i -∗
+    False ;
+
+  ws_hub_create_spec ι sz :
+    (0 ≤ sz)%Z →
+    {{{ True }}}
+      ws_hub_create #sz
+    {{{ t,
+      RET t;
+      ws_hub_inv t ι ∗
+      ws_hub_model t ∅ ∗
+      [∗ list] i ∈ seq 0 (Z.to_nat sz),
+        ws_hub_owner t i
+    }}} ;
+
+  ws_hub_push_spec t ι i v :
+    (0 ≤ i)%Z →
+    <<<
+      ws_hub_inv t ι ∗
+      ws_hub_owner t (Z.to_nat i)
+    | ∀∀ vs,
+      ws_hub_model t vs
+    >>>
+      ws_hub_push t #i v @ ↑ι
+    <<<
+      ws_hub_model t ({[+v+]} ⊎ vs)
+    | RET ();
+      ws_hub_owner t (Z.to_nat i)
+    >>> ;
+
+  ws_hub_push_foreign_spec t ι v :
+    <<<
+      ws_hub_inv t ι
+    | ∀∀ vs,
+      ws_hub_model t vs
+    >>>
+      ws_hub_push_foreign t v @ ↑ι
+    <<<
+      ws_hub_model t ({[+v+]} ⊎ vs)
+    | RET (); True
+    >>> ;
+
+  ws_hub_pop_spec t ι i :
+    (0 ≤ i)%Z →
+    <<<
+      ws_hub_inv t ι ∗
+      ws_hub_owner t (Z.to_nat i)
+    | ∀∀ vs,
+      ws_hub_model t vs
+    >>>
+      ws_hub_pop t #i @ ↑ι
+    <<<
+      ∃∃ o,
+      match o with
+      | None =>
+          ws_hub_model t vs
+      | Some v =>
+          ∃ vs',
+          ⌜vs = {[+v+]} ⊎ vs'⌝ ∗
+          ws_hub_model t vs'
+      end
+    | RET o;
+      ws_hub_owner t (Z.to_nat i)
+    >>> ;
+
+  ws_hub_try_steal_spec t ι i max_round_noyield max_round_yield :
+    (0 ≤ i)%Z →
+    (0 ≤ max_round_noyield)%Z →
+    (0 ≤ max_round_yield)%Z →
+    <<<
+      ws_hub_inv t ι ∗
+      ws_hub_owner t (Z.to_nat i)
+    | ∀∀ vs,
+      ws_hub_model t vs
+    >>>
+      ws_hub_try_steal t #i (#max_round_noyield, #max_round_yield)%V @ ↑ι
+    <<<
+      ∃∃ o,
+      match o with
+      | None =>
+          ws_hub_model t vs
+      | Some v =>
+          ∃ vs',
+          ⌜vs = {[+v+]} ⊎ vs'⌝ ∗
+          ws_hub_model t vs'
+      end
+    | RET o;
+      ws_hub_owner t (Z.to_nat i)
+    >>> ;
+
+  ws_hub_steal_spec t ι i max_round_noyield max_round_yield :
+    (0 ≤ i)%Z →
+    (0 ≤ max_round_noyield)%Z →
+    (0 ≤ max_round_yield)%Z →
+    <<<
+      ws_hub_inv t ι ∗
+      ws_hub_owner t (Z.to_nat i)
+    | ∀∀ vs,
+      ws_hub_model t vs
+    >>>
+      ws_hub_steal t #i (#max_round_noyield, #max_round_yield)%V @ ↑ι
+    <<<
+      ∃∃ v vs',
+      ⌜vs = {[+v+]} ⊎ vs'⌝ ∗
+      ws_hub_model t vs'
+    | RET v;
+      ws_hub_owner t (Z.to_nat i)
+    >>> ;
+}.
+#[global] Arguments ws_hub _ {_} : assert.
+#[global] Arguments Build_ws_hub {_ _ _ _ _ _ _ _ _ _ _ _ _} _ _ _ _ _ _ _ : assert.
+#[global] Opaque ws_hub_create.
+#[global] Opaque ws_hub_push.
+#[global] Opaque ws_hub_push_foreign.
+#[global] Opaque ws_hub_pop.
+#[global] Opaque ws_hub_try_steal.
+#[global] Opaque ws_hub_steal.
+
+Section zebre_G.
+  Context `{zebre_G : !ZebreG Σ}.
+  Context (ws_hub : ws_hub Σ).
+
+  Definition ws_hub_pop_try_steal : val :=
+    λ: "t" "i" "max_round",
+      match: ws_hub.(ws_hub_pop) "t" "i" with
+      | Some <> as "res" =>
+          "res"
+      | None =>
+          ws_hub.(ws_hub_try_steal) "t" "i" "max_round"
+      end.
+
+  Definition ws_hub_pop_steal : val :=
+    λ: "t" "i" "max_round",
+      match: ws_hub.(ws_hub_pop) "t" "i" with
+      | Some "v" =>
+          "v"
+      | None =>
+          ws_hub.(ws_hub_steal) "t" "i" "max_round"
+      end.
+
+  Lemma ws_hub_pop_try_steal_spec t ι i max_round_noyield max_round_yield :
+    (0 ≤ i)%Z →
+    (0 ≤ max_round_noyield)%Z →
+    (0 ≤ max_round_yield)%Z →
+    <<<
+      ws_hub.(ws_hub_inv) t ι ∗
+      ws_hub.(ws_hub_owner) t (Z.to_nat i)
+    | ∀∀ vs,
+      ws_hub.(ws_hub_model) t vs
+    >>>
+      ws_hub_pop_try_steal t #i (#max_round_noyield, #max_round_yield)%V @ ↑ι
+    <<<
+      ∃∃ o,
+      match o with
+      | None =>
+          ws_hub.(ws_hub_model) t vs
+      | Some v =>
+          ∃ vs',
+          ⌜vs = {[+v+]} ⊎ vs'⌝ ∗
+          ws_hub.(ws_hub_model) t vs'
+      end
+    | RET o;
+      ws_hub.(ws_hub_owner) t (Z.to_nat i)
+    >>>.
+  Proof.
+    iIntros "%Hi %Hmax_round_noyield %Hmax_round_yield !> %Φ (#Hinv & Howner) HΦ".
+
+    wp_rec.
+
+    awp_smart_apply (ws_hub_pop_spec with "[$Hinv $Howner]"); [done.. |].
+    iApply (aacc_aupd with "HΦ"); first done. iIntros "%vs Hmodel".
+    iAaccIntro with "Hmodel"; first iSteps. iIntros ([v |]) "Hmodel !>".
+
+    - iRight. iExists (Some v). iFrame.
+      iIntros "HΦ !> Howner". clear.
+
+      iSpecialize ("HΦ" with "Howner").
+      iSteps.
+
+    - iLeft. iFrame.
+      iIntros "HΦ !> Howner". clear- Hi Hmax_round_noyield Hmax_round_yield.
+
+      wp_smart_apply (ws_hub_try_steal_spec with "[$Hinv $Howner] HΦ"); done.
+  Qed.
+
+  Lemma ws_hub_pop_steal_spec t ι i max_round_noyield max_round_yield :
+    (0 ≤ i)%Z →
+    (0 ≤ max_round_noyield)%Z →
+    (0 ≤ max_round_yield)%Z →
+    <<<
+      ws_hub.(ws_hub_inv) t ι ∗
+      ws_hub.(ws_hub_owner) t (Z.to_nat i)
+    | ∀∀ vs,
+      ws_hub.(ws_hub_model) t vs
+    >>>
+      ws_hub_pop_steal t #i (#max_round_noyield, #max_round_yield)%V @ ↑ι
+    <<<
+      ∃∃ v vs',
+      ⌜vs = {[+v+]} ⊎ vs'⌝ ∗
+      ws_hub.(ws_hub_model) t vs'
+    | RET v;
+      ws_hub.(ws_hub_owner) t (Z.to_nat i)
+    >>>.
+  Proof.
+    iIntros "%Hi %Hmax_round_noyield %Hmax_round_yield !> %Φ (#Hinv & Howner) HΦ".
+
+    wp_rec.
+
+    awp_smart_apply (ws_hub_pop_spec with "[$Hinv $Howner]"); [done.. |].
+    iApply (aacc_aupd with "HΦ"); first done. iIntros "%vs Hmodel".
+    iAaccIntro with "Hmodel"; first iSteps. iIntros ([v |]) "Hmodel !>".
+
+    - iDestruct "Hmodel" as "(%vs' & -> & Hmodel)".
+      iRight. iExists v, vs'. iFrame. iStep.
+      iIntros "HΦ !> Howner". clear.
+
+      iSpecialize ("HΦ" with "Howner").
+      iSteps.
+
+    - iLeft. iFrame.
+      iIntros "HΦ !> Howner". clear- Hi Hmax_round_noyield Hmax_round_yield.
+
+      wp_smart_apply (ws_hub_steal_spec with "[$Hinv $Howner] HΦ"); done.
+  Qed.
+End zebre_G.
+
+#[global] Opaque ws_hub_pop_try_steal.
+#[global] Opaque ws_hub_pop_steal.
